Fix up SimAsm analysis

SimAsm/Examples/PetersonLitmus.thy
@@ -1,17 +1,96 @@
 theory PetersonLitmus
-  imports "../SimAsm_Syntax" "../SimAsm_Inter"
+  imports "../SimAsm_Syntax" 
 begin
 
 datatype globals = X | Y | T
 record aux = S :: bool
 
-theorem upd_correct:
-  assumes "upd2 R (lift\<^sub>c c) P \<subseteq> {p. point.inv p}"
-  shows "rif (step\<^sub>t R) (step G) (lift\<^sub>c c)"
-  sorry
+(*
+definition Rtest
+  where "Rtest = \<llangle>((\<^sup>1\<lbrakk>X\<rbrakk> \<longrightarrow> \<^sup>2\<^sup>aS \<longrightarrow> \<^sup>1\<^sup>aS) \<and> \<^sup>1\<lbrakk>X\<rbrakk> = \<^sup>2\<lbrakk>X\<rbrakk> \<and> (\<^sup>2\<lbrakk>T\<rbrakk> = \<^sup>1\<lbrakk>T\<rbrakk> \<or> (\<^sup>1\<lbrakk>T\<rbrakk> \<and> \<not> \<^sup>2\<lbrakk>T\<rbrakk> \<and> (\<^sup>1\<lbrakk>X\<rbrakk> \<longrightarrow> \<not>\<^sup>2\<^sup>aS))))\<rrangle>"
 
-instance aux_ext :: (equal) equal
-  by standard
+lemma reg_assign [simp]:
+  "((\<lambda>v. (v = n \<longrightarrow> st m' e) \<and> (v \<noteq> n \<longrightarrow> st m' (Reg v))) = (\<lambda>v. st x (Reg v))) = 
+   (st x (Reg n) = st m' e \<and> (\<forall>v. v \<noteq> n \<longrightarrow> st x (Reg v) = st m' (Reg v)))"
+  apply auto
+  apply metis
+  apply metis
+  apply metis
+  apply metis
+  done
+
+lemma reg_assign' [simp]:
+  "((\<lambda>v. ((v::nat) = 0 \<longrightarrow> st m' e) \<and> (0 < v \<longrightarrow> st m' (Reg v))) = (\<lambda>v. st x (Reg v))) = 
+   (st x (Reg 0) = st m' e \<and> (\<forall>v. 0 < v \<longrightarrow> st x (Reg v) = st m' (Reg v)))"
+proof -
+  have "((\<lambda>v. ((v::nat) = 0 \<longrightarrow> st m' e) \<and> (0 < v \<longrightarrow> st m' (Reg v))) = (\<lambda>v. st x (Reg v))) = 
+        ((\<lambda>v. (v = 0 \<longrightarrow> st m' e) \<and> (v \<noteq> 0 \<longrightarrow> st m' (Reg v))) = (\<lambda>v. st x (Reg v)))"
+    by auto
+  also have "... = (st x (Reg 0) = st m' e \<and> (\<forall>v. v \<noteq> 0 \<longrightarrow> st x (Reg v) = st m' (Reg v)))"
+    using reg_assign[of 0 m' e x] by blast
+  also have "... = (st x (Reg 0) = st m' e \<and> (\<forall>v. 0 < v \<longrightarrow> st x (Reg v) = st m' (Reg v)))"
+    by simp
+  finally show ?thesis .
+qed
+
+lemma
+  "stable\<^sub>t Rtest P \<Longrightarrow>
+   sp (sp P (\<^bold>r(0 :: nat) := \<lbrakk>Y\<rbrakk> :\<^sub>a \<^sup>aS := (\<^sup>aS \<and> \<^sup>0\<lbrakk>Y\<rbrakk>)) Rtest) (\<^bold>r1 := \<lbrakk>T\<rbrakk>) Rtest \<subseteq> 
+   sp (sp P (\<^bold>r1 := \<lbrakk>T\<rbrakk>) Rtest) (\<^bold>r0 := \<lbrakk>Y\<rbrakk> :\<^sub>a \<^sup>aS := (\<^sup>aS \<and> \<^sup>0\<lbrakk>Y\<rbrakk>)) Rtest"
+  apply (clarsimp simp: step\<^sub>t_def aux_upd_def glb_def rg_def Rtest_def st_upd_def)
+  apply (rename_tac m\<^sub>3 m\<^sub>2 m\<^sub>1)
+  apply (intro exI conjI impI)
+  apply (subgoal_tac "m\<^sub>2 (Reg 0 :=\<^sub>s st m\<^sub>1 (Reg 0)) \<in> P")
+  apply (thin_tac "m\<^sub>1 \<in> P")
+  apply blast
+  defer 1
+  prefer 4
+  apply (subgoal_tac "st (m\<^sub>3(Glb Y :=\<^sub>s st m\<^sub>1 (Glb Y), Reg 0 :=\<^sub>s st m\<^sub>1 (Reg 0))) (Reg (Suc 0)) = 
+                      st (m\<^sub>2(Reg 0 :=\<^sub>s st m\<^sub>1 (Reg 0))) (Glb T)")
+  apply blast
+  apply (clarsimp simp: st_upd_def)+
+
+  apply (subgoal_tac "(m\<^sub>1, m\<^sub>2\<lparr>st := (st m\<^sub>2)(Reg 0 := st m\<^sub>1 (Reg 0))\<rparr>) \<in> {(m, m').
+         (st m (Glb X) \<longrightarrow> S (state_rec.more m') \<longrightarrow> S (state_rec.more m)) \<and>
+         st m (Glb X) = st m' (Glb X) \<and>
+         (st m' (Glb T) = st m (Glb T) \<or>
+          st m (Glb T) \<and>
+          \<not> st m' (Glb T) \<and> (st m (Glb X) \<longrightarrow> \<not> S (state_rec.more m'))) \<and>
+         (\<lambda>v. st m (Reg v)) = (\<lambda>v. st m' (Reg v))}") 
+  unfolding stable_def apply presburger
+  by auto
+
+lemma
+  "stable\<^sub>t Rtest P \<Longrightarrow>
+   sp (sp P (\<^bold>r1 := \<lbrakk>T\<rbrakk>) Rtest) (\<^bold>r0 := \<lbrakk>Y\<rbrakk> :\<^sub>a \<^sup>aS := (\<^sup>aS \<and> \<^sup>0\<lbrakk>Y\<rbrakk>)) Rtest \<subseteq>
+   sp (sp P (\<^bold>r(0 :: nat) := \<lbrakk>Y\<rbrakk> :\<^sub>a \<^sup>aS := (\<^sup>aS \<and> \<^sup>0\<lbrakk>Y\<rbrakk>)) Rtest) (\<^bold>r1 := \<lbrakk>T\<rbrakk>) Rtest"
+  apply (clarsimp simp: step\<^sub>t_def aux_upd_def glb_def rg_def Rtest_def st_upd_def)
+  apply (rename_tac m\<^sub>3 m\<^sub>2 m\<^sub>1)
+  apply (intro exI conjI impI)
+  apply (subgoal_tac "m\<^sub>2(Reg 1 :=\<^sub>s st m\<^sub>1 (Reg 1), Glb T :=\<^sub>s st m\<^sub>1 (Glb T)) \<in> P")
+  apply (thin_tac "m\<^sub>1 \<in> P")
+  apply blast
+  defer 1
+  prefer 5
+  apply (subgoal_tac "st (m\<^sub>3(Reg 1 :=\<^sub>s st m\<^sub>1 (Reg 1), Glb T :=\<^sub>s st m\<^sub>1 (Glb T))) (Reg 0) = 
+                      st (m\<^sub>2(Reg 1 :=\<^sub>s st m\<^sub>1 (Reg 1), Glb T :=\<^sub>s st m\<^sub>1 (Glb T))) (Glb Y)")
+  apply blast
+  apply (clarsimp simp: st_upd_def)+
+  apply blast
+  apply (clarsimp simp: st_upd_def)+
+
+  apply (subgoal_tac "(m\<^sub>1, m\<^sub>2\<lparr>st := (st m\<^sub>2)
+             (Reg (Suc 0) := st m\<^sub>1 (Reg (Suc 0)), Glb T := st m\<^sub>1 (Glb T))\<rparr>) \<in> {(m, m').
+         (st m (Glb X) \<longrightarrow> S (state_rec.more m') \<longrightarrow> S (state_rec.more m)) \<and>
+         st m (Glb X) = st m' (Glb X) \<and>
+         (st m' (Glb T) = st m (Glb T) \<or>
+          st m (Glb T) \<and>
+          \<not> st m' (Glb T) \<and> (st m (Glb X) \<longrightarrow> \<not> S (state_rec.more m'))) \<and>
+         (\<lambda>v. st m (Reg v)) = (\<lambda>v. st m' (Reg v))}") 
+  unfolding stable_def apply presburger
+  apply clarsimp
+  by blast
+*)
 
 lemma thread0:
   "FNBEGIN
@@ -22,7 +101,7 @@ lemma thread0:
       \<lbrakk>X\<rbrakk> := #True;
       fence;
       \<lbrakk>T\<rbrakk> := #True :\<^sub>a \<^sup>aS := True;
-fence;
+      fence;
       \<^bold>r0 := \<lbrakk>Y\<rbrakk> :\<^sub>a \<^sup>aS := (\<^sup>aS \<and> \<^sup>0\<lbrakk>Y\<rbrakk>);
       \<^bold>r1 := \<lbrakk>T\<rbrakk>
     }
@@ -39,15 +118,14 @@ fence;
   (* Guarantees of each atomic action *)
   apply (auto simp: wp\<^sub>r_def st_upd_def step_def glb_def aux_upd_def)[1]
 
+  (* WP *)
   apply simp
   apply (clarsimp simp: stabilize_def st_upd_def glb_def aux_upd_def rg_def)
   apply (meson less_numeral_extra(3))
 
-  apply (rule upd_correct[where ?P="{}"])
-
-  apply (simp add: upd\<^sub>a_def gen_def liftg_def liftl_def)
-
-  apply (clarsimp simp: aux_upd_def st_upd_def stabilize_def glb_def rg_def)[1]
+  (* RIF *)
+  apply rif_eval
+  apply (clarsimp simp: checks_def)
   sorry
 
 lemma thread1:
@@ -57,7 +135,9 @@ lemma thread1:
     P: True
     {
       \<lbrakk>Y\<rbrakk> := #True;
+      fence;
       \<lbrakk>T\<rbrakk> := #False :\<^sub>a \<^sup>aS := False;
+      fence;
       \<^bold>r0 := \<lbrakk>X\<rbrakk> :\<^sub>a \<^sup>aS := (\<^sup>aS \<or> \<not>\<^sup>0\<lbrakk>X\<rbrakk>);
       \<^bold>r1 := (!\<lbrakk>T\<rbrakk>)
     }
@@ -74,11 +154,17 @@ lemma thread1:
   (* Guarantees of each atomic action *)
   apply (auto simp: wp\<^sub>r_def st_upd_def step_def glb_def aux_upd_def)[1]
 
+  (* WP *)
   apply simp
   apply (clarsimp simp: stabilize_def st_upd_def glb_def aux_upd_def rg_def c_neg_def)
   apply (intro conjI impI)
-  defer 1
+  prefer 2
   apply (meson less_numeral_extra(3))
-  by auto
+  apply auto[1]
+
+  (* RIF *)
+  apply rif_eval
+  apply (clarsimp simp: checks_def)
+  sorry
 
 end
