SimAsm/SimAsm_Inter.thy
@@ -1,180 +1,394 @@
 theory SimAsm_Inter
-  imports SimAsm_WP "HOL-Library.While_Combinator"
+  imports "HOL-Library.FSet" SimAsm_WP "HOL-Library.While_Combinator" "HOL-Eisbach.Eisbach"
 begin
 
-record ('v,'g,'r,'a) point =
-  op  :: "('v,'g,'r,'a) opbasic"
-  rgs :: "'r set"          
-  wrs :: "'g set"
-  rds :: "'g set"
-  fen :: bool
-  inv :: bool
+text \<open>A data point, extends an instruction with reordering information\<close>
+record ('g,'r) point =
+  id :: nat
+  wrs :: "('g,'r) var fset"
+  rds :: "('g,'r) var fset"
+  bar :: bool
+  pairs :: "nat fset"
 
-fun upd_assign
-  where 
-    "upd_assign (Reg r) e p = p" |
-    "upd_assign (Glb g) e p = p"
-
-fun upd_cmp
-  where
-    "upd_cmp b p = p"
-
-abbreviation shr
-  where "shr A \<equiv> {g. Glb g \<in> A}"
-
-abbreviation priv
-  where "priv A \<equiv> {g. Reg g \<in> A}"
+type_synonym ('v,'g,'r,'a) enumi = "('v,'g,'r,'a) pred \<times> ('v,'g,'r) op \<times> ('v,'g,'r,'a) auxfn"
+type_synonym ('v,'g,'r,'a) enuml = "('v,'g,'r,'a) enumi list"
 
 abbreviation inst
   where "inst a \<equiv> fst (tag a)"
 
+definition point_cmp (infix "\<prec>" 60)
+  where "point_cmp a b \<equiv> wrs a |\<subseteq>| wrs b \<and> rds a |\<subseteq>| rds b \<and> (bar a \<longrightarrow> bar b)"
+
+fun fences
+  where "fences full_fence = True" | "fences _ = False"
+
+definition hasGlobal
+  where "hasGlobal S \<equiv> \<exists>e. Glb e |\<in>| S"
+
+fun hasGlobalL
+  where "hasGlobalL (Glb x#a) = True" | 
+        "hasGlobalL [] = False" |
+        "hasGlobalL (b#a) = hasGlobalL a"
+
+lemma [intro]: "finite (deps a)" by (induct a, auto)
+lemma [intro]: "finite (deps\<^sub>B a)" by (induct a, auto)
+lemma [intro]: "finite (wr a)" by (induct a, auto)
+lemma [intro]: "finite (rd a)" by (induct a, auto)
+
+text \<open>Substitute a variable for an expression\<close>
+fun subst :: "('v,'g,'r) exp \<Rightarrow> ('g,'r) var \<Rightarrow> ('v,'g,'r) exp \<Rightarrow> ('v,'g,'r) exp"
+  where
+    "subst (Var r) r' e = (if r = r' then e else Var r)" |
+    "subst (Exp f rs) r e = (Exp f (map (\<lambda>x. subst x r e) rs))" |
+    "subst e _ _ = e"
+
+text \<open>The syntactic dependencies of an expression\<close>
+fun ldeps :: "('v,'g,'r) exp \<Rightarrow> ('g,'r) var list"
+  where 
+    "ldeps (Var r) = [r]" |
+    "ldeps (Exp _ rs) = List.bind rs ldeps" |
+    "ldeps _ = []"
+
+fun ldeps\<^sub>B :: "('v,'g,'r) bexp \<Rightarrow> ('g,'r) var list"
+  where 
+    "ldeps\<^sub>B (Neg e) = ldeps\<^sub>B e" |
+    "ldeps\<^sub>B (Exp\<^sub>B _ rs) = List.bind rs ldeps"
+
+definition fdeps 
+  where "fdeps a = fset_of_list (ldeps a)"
+
+definition fdeps\<^sub>B
+  where "fdeps\<^sub>B a = fset_of_list (ldeps\<^sub>B a)"
+
+text \<open>Variables written by an operation\<close>
+fun fwr :: "('v,'g,'r) op \<Rightarrow> ('g,'r) var fset"
+  where 
+    "fwr (assign y _) = {|y|}" |
+    "fwr _ = {||}"
+
+text \<open>Variables read by an operation\<close>
+fun frd :: "('v,'g,'r) op \<Rightarrow> ('g,'r) var fset"
+  where
+    "frd (assign _ e) = fdeps e" |
+    "frd (cmp b) = fdeps\<^sub>B b" |
+    "frd _ = {||}"
+
+text \<open>Conditions under which a point is ordered after an instruction\<close>
 fun ord
   where
-    "ord nop p = False" |
-    "ord (cmp b) p = (wrs p \<noteq> {} \<or> shr (deps\<^sub>B b) \<inter> rds p \<noteq> {})" |
-    "ord (assign (Reg r) e) p = (shr (deps e) \<inter> (rds p \<union> wrs p) \<noteq> {} \<or> (r \<in> rgs p \<and> shr (deps e) \<noteq> {}))" |
-    "ord (assign (Glb x) e) p = (shr (deps e) \<inter> (rds p \<union> wrs p) \<noteq> {} \<or> x \<in> wrs p)" |
+    "ord nop p = (bar p)" |
+    "ord (cmp b) p = (bar p \<or> hasGlobal (wrs p) \<or> hasGlobal (fdeps\<^sub>B b |\<inter>| rds p))" |
+    "ord (assign v e) p = 
+      (bar p \<or> 
+        hasGlobal (fdeps e |\<inter>| (rds p |\<union>| wrs p)) \<or> 
+        (case v of Glb g \<Rightarrow> Glb g |\<in>| wrs p | _ \<Rightarrow> False) \<or> 
+        (hasGlobal (fdeps e) \<and> v |\<in>| rds p))" |
     "ord full_fence _ = True"
 
-fun wp\<^sub>b :: "('v,'g,'a) grel \<Rightarrow> ('v,'g,'r,'a) opbasic \<Rightarrow> ('v,'g,'r,'a) trans"
-  where "wp\<^sub>b R ((\<alpha>,f),v,_) Q = stabilize R (v \<inter> wp\<^sub>i \<alpha> (wp\<^sub>a f Q))"
-
-fun chk :: "('v,'g,'a) grel \<Rightarrow> ('v,'g,'r,'a) opbasic \<Rightarrow> ('v,'g,'r,'a) point \<Rightarrow> bool"
+text \<open>Strengthen a point based on a strictly earlier instruction\<close>
+fun stren :: "('v,'g,'r) op \<Rightarrow> ('g,'r) point \<Rightarrow> ('g,'r) point"
   where
-    "chk R a p = 
-      (inst a = full_fence \<or>
-      (\<forall>Q. stable\<^sub>t R Q \<longrightarrow> wp\<^sub>b Id a (wp\<^sub>b R (op p) Q) \<subseteq> wp\<^sub>b Id (op p) (wp\<^sub>b R a Q)))"
+    "stren a p = p\<lparr> wrs := wrs p |\<union>| fwr a, 
+                    rds := rds p |\<union>| frd a, 
+                    bar := bar p \<or> fences a \<rparr>"
 
-fun stren :: "('v,'g,'r) op \<Rightarrow> ('v,'g,'r,'a) point \<Rightarrow> ('v,'g,'r,'a) point"
+text \<open>Weaken a point based on a reorderable instruction\<close>
+fun wken :: "nat \<Rightarrow> ('v,'g,'r) op \<Rightarrow> ('g,'r) point \<Rightarrow> ('g,'r) point"
   where
-    "stren a p = p\<lparr> rgs := rgs p - priv (wr a) \<union> priv (rd a), 
-                    wrs := wrs p \<union> shr (wr a), 
-                    rds := rds p \<union> shr (rd a), 
-                    fen := fen p \<or> (a = full_fence) \<rparr>"
+    "wken n \<alpha> p = p\<lparr> rds := rds p - fwr \<alpha> |\<union>| 
+                            (if fwr \<alpha> |\<inter>| rds p \<noteq> {||} then frd \<alpha> else {||}), 
+                     pairs := pairs p |\<union>| {|n|} \<rparr>"
 
-fun weaken :: "('v,'g,'r) op \<Rightarrow> ('v,'g,'r,'a) point \<Rightarrow> ('v,'g,'r,'a) point"
+text \<open>Convert an instruction into a point\<close>
+definition gen :: "nat \<Rightarrow> ('v,'g,'r) op \<Rightarrow> ('g,'r) point"
   where
-    "weaken a p = p\<lparr> rds := rds p - shr (wr a), op := fwd\<^sub>s (op p) (a,state_rec.more) \<rparr>"
+    "gen n a = \<lparr> id = n, wrs = fwr a, rds = frd a, bar = fences a, pairs = {||} \<rparr>"
 
-fun upd\<^sub>i
+text \<open>Process a new instruction against one point\<close>
+definition proc1 :: "nat \<Rightarrow> ('v,'g,'r) op \<Rightarrow> ('g,'r) point \<Rightarrow> ('g,'r) point"
   where
-    "upd\<^sub>i R a p = (if fen p \<or> ord (inst a) p then stren (inst a) p 
-                  else (weaken (inst a) p)\<lparr>inv := inv p \<and> chk R a p\<rparr>)"
+    "proc1 n \<alpha> p \<equiv> if ord \<alpha> p then stren \<alpha> p else wken n \<alpha> p"
 
-definition gen
-  where
-    "gen a = \<lparr> op = a, 
-              rgs = priv (rd (inst a)), 
-              wrs = shr (wr (inst a)), 
-              rds = shr (rd (inst a)), 
-              fen = (inst a = full_fence),
-              inv = True\<rparr>"
-
-definition upd\<^sub>a
-  where "upd\<^sub>a R a P = ({ gen a } \<union> ((upd\<^sub>i R a) ` P))"
-
-fun upd2
+text \<open>Process a new instruction against a set of points\<close>
+definition proc\<^sub>i :: "nat \<Rightarrow> ('v,'g,'r) op \<Rightarrow> ('g,'r) point set \<Rightarrow> ('g,'r) point set"
   where 
-    "upd2 R (Basic a) P = upd\<^sub>a R a P" |
-    "upd2 R (Choice c\<^sub>1 c\<^sub>2) P = (upd2 R c\<^sub>1 P \<union> upd2 R c\<^sub>2 P)" |
-    "upd2 R (Loop c) P = lfp (\<lambda>Y. (P \<union> upd2 R c Y))" |
-    "upd2 R (c\<^sub>1 ;; c\<^sub>2) P = upd2 R c\<^sub>1 (upd2 R c\<^sub>2 P)" |
-    "upd2 R _ P = P"
+    "proc\<^sub>i n a P \<equiv> proc1 n a ` P"
 
-declare upd2.simps(3)[simp del]
+fun enum :: "('v,'g,'r,'a) lang \<Rightarrow> ('v,'g,'r,'a) enuml \<Rightarrow> (nat, nat) com \<times> ('v,'g,'r,'a) enuml"
+  where
+    "enum Skip l = (com.Nil,l)" |
+    "enum (Op v a f) l = (Basic (length l,{},{}),l@[(v,a,f)])" |
+    "enum (Seq c\<^sub>1 c\<^sub>2) l = 
+      (case enum c\<^sub>2 l of (n\<^sub>2,l) \<Rightarrow> (case enum c\<^sub>1 l of (n\<^sub>1,l) \<Rightarrow> (com.Seq n\<^sub>1 n\<^sub>2,l)))" |
+    "enum (If b c\<^sub>1 c\<^sub>2) l = 
+      (case enum c\<^sub>2 l of (n\<^sub>2,l) \<Rightarrow> case enum c\<^sub>1 l of (n\<^sub>1,l) \<Rightarrow> 
+        (Choice (com.Seq (Basic (length l,{},{})) n\<^sub>1) (com.Seq (Basic (length l,{},{})) n\<^sub>2),
+          l@[({},cmp b,state_rec.more)]))" |
+    "enum (While b I c) l = 
+      (case enum c l of (n,l) \<Rightarrow> 
+        (com.Seq ((com.Seq (Basic (length l,{},{})) n)*) (Basic (length l,{},{}))),
+          l@[({},cmp b,state_rec.more)])" |
+    "enum (DoWhile I c b) l = 
+      (case enum c l of (n,l) \<Rightarrow> 
+        ((n ;; Basic (length l,{},{}))* ;; n ;; Basic (length l,{},{}), 
+          l@[({},cmp b,state_rec.more)]))" 
 
-lemma mono_upd\<^sub>a:
-  "mono (upd\<^sub>a R a)"
-  by (smt Un_mono image_Un monoI order_refl sup.orderE sup_ge2 upd\<^sub>a_def)
+text \<open>Process a full program, but don't introduce new actions. Used only for reasoning\<close>
+fun proc :: "(nat, nat) com \<Rightarrow> ('v,'g,'r,'a) enuml \<Rightarrow> ('g,'r) point set \<Rightarrow> ('g,'r) point set"
+  where 
+    "proc (Basic a) l P = proc\<^sub>i (tag a) (fst (snd (l ! (tag a)))) P" |
+    "proc (Choice c\<^sub>1 c\<^sub>2) l P = (proc c\<^sub>1 l P \<union> proc c\<^sub>2 l P)" |
+    "proc (Loop c) l P = lfp (\<lambda>Y. (P \<union> proc c l Y))" |
+    "proc (c\<^sub>1 ;; c\<^sub>2) l P = proc c\<^sub>1 l (proc c\<^sub>2 l P)" |
+    "proc _ _ P = P"
 
-lemma mono_upd:
-  "mono (upd2 R c)"
+text \<open>Process a new instruction against a set of points\<close>
+definition rif\<^sub>i :: "nat \<Rightarrow> ('v,'g,'r) op \<Rightarrow> ('g,'r) point set \<Rightarrow> ('g,'r) point set"
+  where 
+    "rif\<^sub>i n a P \<equiv> { gen n a } \<union> proc\<^sub>i n a P"
+
+text \<open>Process a full program\<close>
+fun rif :: "(nat, nat) com \<Rightarrow> ('v,'g,'r) op list \<Rightarrow> ('g,'r) point set \<Rightarrow> ('g,'r) point set"
+  where 
+    "rif (Basic a) l P = (if tag a < length l then rif\<^sub>i (tag a) (l ! (tag a)) P else P)" |
+    "rif (Choice c\<^sub>1 c\<^sub>2) l P = (rif c\<^sub>1 l P \<union> rif c\<^sub>2 l P)" |
+    "rif (Loop c) l P = lfp (\<lambda>Y. (P \<union> rif c l Y))" |
+    "rif (c\<^sub>1 ;; c\<^sub>2) l P = rif c\<^sub>1 l (rif c\<^sub>2 l P)" |
+    "rif _ _ P = P"
+declare rif.simps(3)[simp del]
+
+text \<open>Interference Check\<close>
+fun sp 
+  where 
+    "sp P (v,i,a) R = {m. \<exists>m' m''. m' \<in> P \<and> (m',m'') \<in> beh\<^sub>i i \<and> (m''(aux: a),m) \<in> step\<^sub>t R}"
+ 
+definition chk 
+  where
+    "chk a b R = (\<forall>P. stable\<^sub>t R P \<longrightarrow> sp (sp P a R) b R  \<subseteq> sp (sp P b R) a R)"
+
+definition checks 
+  where "checks l P R \<equiv> \<forall>p \<in> P. \<forall>i. i |\<in>| pairs p \<longrightarrow> chk (l ! i) (l ! id p) R"
+
+definition rif_full
+  where "rif_full c \<equiv> case enum c [] of (n,l) \<Rightarrow> (rif n (map (fst o snd) l) {},l)"
+
+definition rif_checks
+  where "rif_checks c R \<equiv> case rif_full c of (n,l) \<Rightarrow> checks l n R"
+
+section \<open>Soundness\<close>
+
+lemma mono_proc\<^sub>i:
+  "mono (proc\<^sub>i n a)"
+  by (smt Un_mono image_Un monoI order_refl sup.orderE sup_ge2 proc\<^sub>i_def)
+
+lemma mono_rif\<^sub>i:
+  "mono (rif\<^sub>i n a)"
+  by (smt Un_mono monoI mono_Un mono_proc\<^sub>i rif\<^sub>i_def subset_Un_eq subset_refl sup.bounded_iff)
+
+lemma mono_proc:
+  "mono (proc c l)"
 proof (induct c)
   case (Seq c1 c2)
   then show ?case by (simp add: mono_def)
 next
   case (Choice c1 c2)
   then show ?case
-    by (smt Un_mono mono_def upd2.simps(2))
+    by (smt Un_mono mono_def proc.simps(2))
 next
   case (Loop c)
   then show ?case 
-    by (smt Un_iff lfp_mono monoI subset_eq upd2.simps(3))
-qed (simp add: monoI mono_upd\<^sub>a)+
+    by (smt Un_iff lfp_mono monoI subset_eq proc.simps(3))
+qed (simp add: monoI mono_proc\<^sub>i)+
 
-lemma mono_union_upd2:
-  "mono (\<lambda>Y. (P \<union> upd2 R c Y))"
-  by (smt Un_mono monoD monoI mono_upd sup.idem sup.order_iff)
+lemma mono_rif:
+  "mono (rif c l)"
+proof (induct c)
+  case (Basic x)
+  then show ?case by (cases "tag x < length l") (auto simp add: monoI mono_rif\<^sub>i)
+next
+  case (Seq c1 c2)
+  then show ?case by (simp add: mono_def)
+next
+  case (Choice c1 c2)
+  then show ?case
+    by (smt Un_mono mono_def rif.simps(2))
+next
+  case (Loop c)
+  then show ?case 
+    by (smt Un_iff lfp_mono monoI subset_eq rif.simps(3))
+qed (simp add: monoI mono_rif\<^sub>i)+
 
+lemma lfp_const [intro]:
+  "x \<in> P \<longrightarrow> x \<in> lfp (\<lambda>Y. P \<union> f Y)"
+  by (meson Un_subset_iff basic_trans_rules(31) lfp_greatest)
+
+lemma lfp_fn [intro]:
+  "mono f \<Longrightarrow> x \<in> f (lfp (\<lambda>Y. Q \<union> f Y)) \<Longrightarrow> x \<in> lfp (\<lambda>Y. Q \<union> f Y)" 
+proof -
+  assume a1: "x \<in> f (lfp (\<lambda>Y. Q \<union> f Y))"
+  assume a2: "mono f"
+  have f3: "\<forall>A. mono ((\<union>) (A::'a set))"
+    by (meson Un_mono monoI subset_refl)
+  then have "x \<in> lfp (\<lambda>A. f (Q \<union> A))"
+    using a2 a1 by (simp add: lfp_rolling)
+  then show ?thesis
+    using f3 a2 lfp_rolling by blast
+qed
+
+lemma mono_union_rif:
+  "mono (\<lambda>Y. (P \<union> rif c l Y))"
+  by (smt Un_mono monoD monoI mono_rif sup.idem sup.order_iff)
+
+lemma [simp]:
+  "proc r l (P \<union> Q) = proc r l P \<union> proc r l Q"
+proof (induct r arbitrary: P Q)
+  case (Loop r)
+  have p: "lfp (\<lambda>Y. P \<union> Q \<union> proc r l Y) \<supseteq> lfp (\<lambda>Y. P \<union> proc r l Y)"
+    apply (rule lfp_mono)
+    by auto
+  have q: "lfp (\<lambda>Y. P \<union> Q \<union> proc r l Y) \<supseteq> lfp (\<lambda>Y. Q \<union> proc r l Y)"
+    apply (rule lfp_mono)
+    by auto
+  hence a: "lfp (\<lambda>Y. P \<union> Q \<union> proc r l Y) \<supseteq> lfp (\<lambda>Y. Q \<union> proc r l Y) \<union> lfp (\<lambda>Y. P \<union> proc r l Y)" (is "?L \<supseteq> ?R")
+    using p by auto
+  hence lr: "?L \<inter> ?R = ?R" by blast
+  have "lfp (\<lambda>Y. Q \<union> proc r l Y) \<union> lfp (\<lambda>Y. P \<union> proc r l Y) \<supseteq> lfp (\<lambda>Y. P \<union> Q \<union> proc r l Y)"
+    apply (rule lfp_induct)
+    unfolding lr Loop
+    apply auto
+    apply (smt Loop.hyps Un_mono monoI subset_Un_eq sup.idem)
+    using lfp_const apply fast
+     using lfp_const apply fast
+     using lfp_fn mono_proc apply fast
+     using lfp_fn mono_proc apply fast
+    done
+  then show ?case unfolding proc.simps using a by blast
+qed (auto simp: proc\<^sub>i_def)
+
+lemma [simp]:
+  "rif r l (P \<union> Q) = rif r l P \<union> rif r l Q"
+proof (induct r arbitrary: P Q)
+  case (Loop r)
+  have p: "lfp (\<lambda>Y. P \<union> Q \<union> rif r l Y) \<supseteq> lfp (\<lambda>Y. P \<union> rif r l Y)"
+    apply (rule lfp_mono)
+    by auto
+  have q: "lfp (\<lambda>Y. P \<union> Q \<union> rif r l Y) \<supseteq> lfp (\<lambda>Y. Q \<union> rif r l Y)"
+    apply (rule lfp_mono)
+    by auto
+  hence a: "lfp (\<lambda>Y. P \<union> Q \<union> rif r l Y) \<supseteq> lfp (\<lambda>Y. Q \<union> rif r l Y) \<union> lfp (\<lambda>Y. P \<union> rif r l Y)" (is "?L \<supseteq> ?R")
+    using p by auto
+  hence lr: "?L \<inter> ?R = ?R" by blast
+  have "lfp (\<lambda>Y. Q \<union> rif r l Y) \<union> lfp (\<lambda>Y. P \<union> rif r l Y) \<supseteq> lfp (\<lambda>Y. P \<union> Q \<union> rif r l Y)"
+    apply (rule lfp_induct)
+    unfolding lr Loop
+    apply auto
+    apply (smt Loop.hyps Un_mono monoI subset_Un_eq sup.idem)
+    using lfp_const apply fast
+    using lfp_const apply fast
+     using lfp_fn mono_rif apply fast
+     using lfp_fn mono_rif apply fast
+    done
+  then show ?case unfolding rif.simps using a by blast
+qed (auto simp: rif\<^sub>i_def proc\<^sub>i_def)
+
+lemma rif_split:
+  "rif r l P = proc r l P \<union> rif r l {}"
+proof (induct r arbitrary: P)
+  case (Seq r1 r2)
+  show ?case 
+    using Seq(2)[of P] Seq(1)[of "rif r2 l P"] Seq(1)[of "rif r2 l {}"]
+    apply simp by blast
+next
+  case (Choice r1 r2)
+  then show ?case unfolding rif.simps proc.simps by blast
+next
+  case (Loop r)
+  have p: "lfp (\<lambda>Y. P \<union> rif r l Y) \<supseteq> lfp (\<lambda>Y. P \<union> proc r l Y)" (is "?L \<supseteq> ?R1")
+    apply (rule lfp_mono)
+    using Loop by blast
+  have q: "lfp (\<lambda>Y. P \<union> rif r l Y) \<supseteq> lfp (\<lambda>Y. {} \<union> rif r l Y)" (is "?L \<supseteq> ?R2")
+    apply (rule lfp_mono)
+    by auto
+  hence a: "?L \<supseteq> ?R1 \<union> ?R2" (is "?L \<supseteq> ?R") using p by auto
+  hence lr: "?L \<inter> ?R = ?R" by blast
+  have "?R \<supseteq> ?L"
+    apply (rule lfp_induct)
+    unfolding lr
+    apply (simp add: mono_union_rif)
+    apply auto
+    using lfp_const apply fast
+    defer 1
+    using lfp_unfold mono_rif apply blast
+    unfolding Loop[of "lfp (\<lambda>Y. P \<union> proc r l Y)"]
+    apply auto
+     using lfp_fn mono_proc apply fast
+    by (metis Loop.hyps UnCI lfp_unfold mono_rif)
+  then show ?case unfolding rif.simps proc.simps using a by blast
+qed (auto simp: proc\<^sub>i_def rif\<^sub>i_def)
+
+(*
 subsection \<open>Correctness\<close>
 
 lemma upd_rw:
   assumes "c \<leadsto> c'" "local c"
-  shows "upd2 R c' P \<subseteq> upd2 R c P"
+  shows "rif c' P \<subseteq> rif c P"
   using assms
 proof (induct arbitrary: P)
   case (seq2 c\<^sub>2 c\<^sub>2' c\<^sub>1)
-  then show ?case by (simp add: monoD mono_upd)
+  then show ?case by (simp add: monoD mono_rif)
 next
   case (loop1 c)
-  then show ?case unfolding upd2.simps
-    using def_lfp_unfold[OF _ mono_union_upd2] by blast
+  then show ?case unfolding rif.simps
+    using def_lfp_unfold[OF _ mono_union_rif] by blast
 next
   case (loop2 c)
-  then show ?case unfolding upd2.simps
-    using def_lfp_unfold[OF _ mono_union_upd2] by blast
+  then show ?case unfolding rif.simps
+    using def_lfp_unfold[OF _ mono_union_rif] by blast
 qed auto
 
-lemma upd_exec:
-  assumes "lexecute c r \<alpha> c'"
-  assumes "\<forall>p \<in> upd2 R c P. inv p"
-  shows "inter\<^sub>c (step\<^sub>t R) (step G) r \<alpha> \<and> (\<forall>p \<in> upd2 R c' P. inv p)"
-  sorry
-
-lemma upd\<^sub>aI1:
+lemma rif\<^sub>i_I:
   assumes "p \<in> P"
-  shows "ord (inst \<alpha>) p \<longrightarrow> stren (inst \<alpha>) p \<in> upd\<^sub>a R \<alpha> P"
-        "\<not> ord (inst \<alpha>) p \<longrightarrow> (weaken (inst \<alpha>) p)\<lparr>inv := inv p \<and> chk R \<alpha> p\<rparr> \<in> upd\<^sub>a R \<alpha> P"
-  using assms unfolding upd\<^sub>a_def by auto
+  shows "ord (inst \<alpha>) p \<longrightarrow> stren \<alpha> p \<in> rif\<^sub>i \<alpha> P"
+        "\<not>ord (inst \<alpha>) p \<longrightarrow> (wken \<alpha> p)\<lparr>inv := inv p \<and> chk \<alpha> (op p)\<rparr> \<in> rif\<^sub>i \<alpha> P"
+  using assms unfolding proc\<^sub>i_def proc1_def rif\<^sub>i_def by auto
 
-lemma inv_orig\<^sub>a [intro]:
-  assumes "\<forall>x\<in>upd\<^sub>a R \<alpha> P. point.inv x" shows "\<forall>p \<in> P. inv p"
+lemma rif\<^sub>i_preserve_inv [intro]:
+  assumes "\<forall> x \<in> rif\<^sub>i \<alpha> P. point.inv x" 
+  shows "\<forall>p \<in> P. inv p"
 proof (clarsimp)
-    fix x assume a: "x \<in> P"
-    show "point.inv x" 
-    proof (cases "ord (inst \<alpha>) x")
-      case True
-      hence "stren (inst \<alpha>) x \<in> upd\<^sub>a R \<alpha> P" using upd\<^sub>aI1[OF a, of \<alpha>] by simp
-      then show ?thesis using assms by auto
-    next
-      case False
-      hence "(weaken (inst \<alpha>) x)\<lparr>inv := inv x \<and> chk R \<alpha> x\<rparr> \<in> upd\<^sub>a R \<alpha> P"
-        using upd\<^sub>aI1[OF a, of \<alpha>] by simp
-      then show ?thesis using assms by auto
-    qed
+  fix x assume a: "x \<in> P"
+  show "point.inv x" 
+  proof (cases "ord (inst \<alpha>) x")
+    case True
+    hence "stren \<alpha> x \<in> rif\<^sub>i \<alpha> P" using rif\<^sub>i_I[OF a, of \<alpha>] by simp
+    then show ?thesis using assms by auto
+  next
+    case False
+    hence "(wken \<alpha> x)\<lparr>inv := inv x \<and> chk R \<alpha> (op x)\<rparr> \<in> rif\<^sub>i \<alpha> P"
+      using rif\<^sub>i_I[OF a, of \<alpha>] by simp
+    then show ?thesis using assms by auto
   qed
+qed 
 
-lemma inv_orig [intro]:
-  assumes "\<forall>p \<in> upd2 R c P. inv p"
+lemma rif_preserve_inv [intro]:
+  assumes "\<forall>p \<in> rif c P. inv p"
   shows "\<forall>p \<in> P. inv p"
   using assms
 proof (induct c arbitrary: P)
   case (Basic x)
-  then show ?case using inv_orig\<^sub>a by fastforce
+  then show ?case using rif\<^sub>i_preserve_inv by fastforce
 next
   case (Seq c1 c2)
-  then show ?case unfolding upd2.simps by blast
+  then show ?case unfolding rif.simps by blast
 next
   case (Choice c1 c2)
-  then show ?case unfolding upd2.simps by blast
+  then show ?case unfolding rif.simps by blast
 next
   case (Loop c)
-  then show ?case unfolding upd2.simps 
-    using lfp_unfold mono_union_upd2 by blast 
-qed (unfold upd2.simps, blast)
+  then show ?case unfolding rif.simps 
+    using lfp_unfold mono_union_rif by blast 
+qed (unfold rif.simps, blast)
 
-definition point_cmp
-  where "point_cmp a b \<equiv> rgs a \<subseteq> rgs b \<and> wrs a \<subseteq> wrs b \<and> rds a \<subseteq> rds b"
 
 lemma point_cmp_refl [intro]:
   "point_cmp a a"
@@ -188,98 +402,46 @@ lemma [simp]:
   "deps\<^sub>B (subst\<^sub>B e r e') = deps\<^sub>B e - {r} \<union> (if r \<in> deps\<^sub>B e then deps e' else {})"
   sorry
 
-
-lemma upd_reorder_com:
-  assumes "reorder_com \<alpha>' c \<alpha>" "p \<in> P" "point_cmp p (gen \<alpha>)" 
-  shows "\<exists>p'. p' \<in> upd2 R c P \<and> op p' = op p \<and> point_cmp p' (gen \<alpha>')"
+lemma ord_sound:
+  assumes "reorder_inst \<alpha>' \<beta> \<alpha>"
+  shows "\<not>ord (inst \<beta>) (gen \<alpha>)"
   using assms
-  sorry (*
-proof (induct rule: reorder_com.induct)
+  apply (cases \<alpha>; cases \<beta>; clarsimp; case_tac a; case_tac aa)
+  by (auto simp: gen_def)
+
+lemma ord_cmp:
+  assumes "\<not>ord \<beta> p'" "p \<prec> p'"
+  shows "\<not>ord \<beta> p"
+  using assms by (cases \<beta>, auto simp: point_cmp_def)
+
+lemma
+  assumes "reorder_com \<alpha>' (Basic \<beta>) \<alpha>" "p \<prec> gen \<alpha>"
+  shows "\<not> ord (inst \<beta>) p"
+  apply (rule ord_cmp)
+  apply (rule ord_sound)
+  using assms by auto
+
+(*
+lemma upd_reorder_com:
+  assumes "reorder_com \<alpha>' c \<alpha>" "p \<in> P" "p \<prec> gen \<alpha>" "op p = \<alpha>"
+  shows "\<exists>p'. p' \<in> rif c P \<and> op p' = \<alpha>' \<and> p' \<prec> gen \<alpha>'"
+  using assms
+proof (induct \<alpha>' c \<alpha> rule: reorder_com.induct)
   case (2 \<alpha>' \<beta> \<alpha>)
-  hence [simp]: "op p = \<alpha>'" by auto
-  have "\<not> ord (inst \<beta>) p"
-    using 2(1,4)
-    apply (cases "inst \<beta>"; cases "tag \<beta>"; cases "\<alpha>'")
-    apply (auto simp: gen_def point_cmp_def)
-    prefer 3
-    apply (subgoal_tac "Glb x \<in> rd aa"; blast)
-    prefer 2
-    apply (subgoal_tac "Glb x \<in> wr aa"; blast)
-    apply (case_tac x11, simp)
-    apply (case_tac aa, simp split: if_splits)
+  hence [simp]: "op p = \<alpha>" by auto
+  have "\<not> ord (inst \<beta>) p" sorry
 
-    apply (elim impE)
-    apply (subgoal_tac "rds p \<subseteq> shr ((deps x12a - {Reg x1} \<union> deps x12))")
-    apply (subgoal_tac "shr (insert (Reg x1) (deps x12)) \<inter> shr (deps x12a - {Reg x1} \<union> deps x12) = {}")
-    apply blast
-    apply blast
-    apply auto[1]
+  hence "(wken \<beta> p)\<lparr>inv := inv p \<and> chk R \<beta> (op p)\<rparr> \<in> proc \<beta> P"
+    using proc_I 2 by blast
 
-    apply (elim conjE exE)
-    apply (subgoal_tac "Glb x \<in> insert (Reg x1) (deps x12)")
-    apply (subgoal_tac "Glb x \<in> (deps x12a - {Reg x1} \<union> deps x12)")
-    apply auto[3]
-
-    apply (elim impE)
-    apply (subgoal_tac "rds p \<subseteq> shr ((deps x12a ))")
-    apply (subgoal_tac "shr ( (deps x12)) \<inter> shr (deps x12a ) = {}")
-    apply blast
-    apply blast
-    apply blast
-
-    apply (elim conjE exE)
-    apply (subgoal_tac "Glb x \<in> insert (Reg x1) (deps x12)")
-    apply (subgoal_tac "Glb x \<in> (deps x12a - {Reg x1} \<union> deps x12)")
-    apply auto[3]
-
-    apply (simp split: if_splits)
-    apply (elim impE)
-
-    apply (subgoal_tac "rds p \<subseteq> shr (deps\<^sub>B x2 - {Reg x1} \<union> deps x12)")
-    apply (subgoal_tac "shr (insert (Reg x1) (deps x12)) \<inter> shr (deps\<^sub>B x2 - {Reg x1} \<union> deps x12) = {}")
-    apply blast
-    apply blast
-    apply auto[1]
-
-    apply (elim conjE exE)
-    apply (subgoal_tac "Glb x \<in> insert (Reg x1) (deps x12)")
-    apply (subgoal_tac "Glb x \<in> (deps\<^sub>B x2 - {Reg x1} \<union> deps x12)")
-    apply auto[3]
-
-    apply (subgoal_tac "rds p \<subseteq> shr (deps\<^sub>B x2 )")
-    apply (subgoal_tac "shr (insert (Reg x1) (deps x12)) \<inter> shr (deps\<^sub>B x2 ) = {}")
-    apply blast
-    apply blast
-    apply auto[1]
-
-    apply simp
-    apply simp
-
-    apply simp
-
-    apply (case_tac aa, simp split: if_splits)
-    apply blast
-    apply blast
-
-    apply (simp split: if_splits)
-    apply blast
-    apply blast
-
-    apply (simp split: if_splits)
-    apply (simp split: if_splits)
-    done
-
-  hence "(weaken (inst \<beta>) p)\<lparr>inv := inv p \<and> chk R \<beta> p\<rparr> \<in> upd\<^sub>a R \<beta> P"
-    using 2 by (auto simp: upd\<^sub>a_def)
-
-  moreover have "point_cmp ((weaken (inst \<beta>) p)\<lparr>inv := inv p \<and> chk R \<beta> p\<rparr>) (gen \<alpha>)"
+  moreover have "(wken \<beta> p)\<lparr>inv := inv p \<and> chk R \<beta> (op p)\<rparr> \<prec> gen \<alpha>'"
     using 2(1,4) unfolding point_cmp_def gen_def
     apply auto
     apply (cases \<alpha>'; cases \<beta>; case_tac a; case_tac aa; case_tac ab; case_tac ac; simp split: if_splits)
     
     sorry
 
-  moreover have "op ((weaken (inst \<beta>) p)\<lparr>inv := inv p \<and> chk R \<beta> p\<rparr>) = \<alpha>'" using 2 by auto
+  moreover have "op ((wken \<beta> p)\<lparr>inv := inv p \<and> chk R \<beta> (op p)\<rparr>) = \<alpha>'" using 2 by auto
 
   ultimately show ?case by auto
 next
@@ -288,35 +450,36 @@ next
     apply simp
     sorry
 qed auto
-*)
+
 
 lemma execute_act:
   assumes "lexecute c r \<alpha> c'"
-  shows "\<exists>p. p \<in> upd2 R c P \<and> op p = \<alpha> \<and> point_cmp p (gen (fwd_com \<alpha> r))"
+  shows "\<exists>p. p \<in> rif c P \<and> op p = (fwd_com \<alpha> r) \<and> point_cmp p (gen (fwd_com \<alpha> r))"
   using assms
 proof (induct arbitrary: P)
   case (act \<alpha>)
-  have "gen \<alpha> \<in> upd\<^sub>a R \<alpha> P" by (auto simp: upd\<^sub>a_def)
+  have "gen \<alpha> \<in> proc \<alpha> P" by (auto simp: proc_def)
   then show ?case by (auto simp: gen_def)
 next
   case (ino c\<^sub>1 r \<alpha> c\<^sub>1' c\<^sub>2)
   then show ?case by simp
 next
   case (ooo c\<^sub>1 r \<alpha> c\<^sub>1' \<alpha>' c\<^sub>2)
-  obtain p where p: "p \<in> upd2 R c\<^sub>1 P" "op p = \<alpha>" "point_cmp p (gen (fwd_com \<alpha> r))"
+  obtain p where p: "p \<in> rif c\<^sub>1 P" "op p = (fwd_com \<alpha> r)" "point_cmp p (gen (fwd_com \<alpha> r))"
     using ooo by blast
   have r: "reorder_com \<alpha>' (c\<^sub>2) (fwd_com \<alpha> r)" using ooo by auto
   then show ?case using p(2) upd_reorder_com[OF r p(1,3), of R] by auto
 qed
 
+(*
 lemma upd_po:
-  assumes "reorder_com \<alpha>' c \<alpha>" "p \<in> P" "point_cmp p (gen \<alpha>)" "\<alpha> = fwd_com (op p) r" "\<forall>a\<in>upd2 R c P. point.inv a"
+  assumes "reorder_com \<alpha>' c \<alpha>" "p \<in> P" "point_cmp p (gen \<alpha>)" "\<alpha> = op p" "\<forall>a \<in> rif c P. point.inv a"
   shows "inter\<^sub>c (step\<^sub>t R) (step G) c \<alpha>"
   using assms
 proof (induct \<alpha>' c \<alpha> arbitrary: P rule: reorder_com.induct)
   case (2 \<alpha>' \<beta> \<alpha>)
   hence "\<not> ord (inst \<beta>) p" sorry (* correctness of ordering analysis *)
-  hence "(weaken (inst \<beta>) p)\<lparr>inv := inv p \<and> chk R \<beta> p\<rparr> \<in> upd\<^sub>a R \<beta> P"
+  hence "(wken (inst \<beta>) p)\<lparr>inv := inv p \<and> chk R \<beta> p\<rparr> \<in> rif \<beta> P"
     using 2(2) unfolding upd\<^sub>a_def upd2.simps upd\<^sub>i.simps by auto
   hence "chk R \<beta> p" using 2 by auto
   then show ?case
@@ -326,10 +489,11 @@ next
   case (3 \<alpha>' c\<^sub>1 c\<^sub>2 \<alpha>)
   then show ?case sorry
 qed auto
+*)
 
 lemma upd_exec':
   assumes "lexecute c r \<alpha> c'"
-  assumes "\<forall>p \<in> upd2 R c P. inv p"
+  assumes "\<forall>p \<in> rif c P. inv p"
   shows "inter\<^sub>c (step\<^sub>t R) (step G) r \<alpha>"
   using assms
 proof (induct arbitrary: P)
@@ -340,72 +504,101 @@ next
   then show ?case by auto
 next
   case (ooo c\<^sub>1 r \<alpha> c\<^sub>1' \<alpha>' c\<^sub>2)
-  then obtain p where p: "p \<in> upd2 R c\<^sub>1 P" "op p = \<alpha>" "point_cmp p (gen (fwd_com \<alpha> r))"
+  then obtain p where p: "p \<in> rif c\<^sub>1 P" "op p = fwd_com \<alpha> r" "point_cmp p (gen (fwd_com \<alpha> r))"
     using execute_act by blast
   have r: "reorder_com \<alpha>' (c\<^sub>2) (fwd_com \<alpha> r)" using ooo by auto
-  have f: "fwd_com \<alpha> r = fwd_com (op p) r" using p by auto
-  have "inter\<^sub>c (step\<^sub>t R) (step G) r \<alpha>" using ooo inv_orig by force
+  have f: "fwd_com \<alpha> r =  (op p) " using p by auto
+  have "inter\<^sub>c (step\<^sub>t R) (step G) r \<alpha>" using ooo rif_preserve_inv by force
   thus ?case using upd_po[OF r p(1,3) f] ooo(4) by auto
 qed
 
 lemma upd\<^sub>aE:
-  assumes "x \<in> upd\<^sub>a R \<alpha> P"
-  obtains (ord) p where "ord (inst \<alpha>) p" "x = stren (inst \<alpha>) p" "p \<in> P" |
-          (ooo) p where "\<not> ord (inst \<alpha>) p" "x = (weaken (inst \<alpha>) p)\<lparr>inv := inv p \<and> chk R \<alpha> p\<rparr>" "p \<in> P" |
+  assumes "x \<in> proc \<alpha> P"
+  obtains (ord) p where "ord (inst \<alpha>) p" "x = stren \<alpha> p" "p \<in> P" |
+          (ooo) p where "\<not> ord (inst \<alpha>) p" "x = (wken \<alpha> p)\<lparr>inv := inv p \<and> chk R \<alpha> (op p)\<rparr>" "p \<in> P" |
           (gen) "x = gen \<alpha>"
 proof -
-  have "x = gen \<alpha> \<or> x \<in> upd\<^sub>i R \<alpha> ` P" using assms by (auto simp: upd\<^sub>a_def)
+  have "x = gen \<alpha> \<or> x \<in> proc1 R \<alpha> ` P" using assms by (auto simp: proc_def)
   thus ?thesis
   proof (elim disjE)
     assume "x = gen \<alpha>"
     thus ?thesis using gen by auto
   next
-    assume "x \<in> upd\<^sub>i R \<alpha> ` P"
-    then obtain p where p: "p \<in> P" "x = upd\<^sub>i R \<alpha> p" by blast
+    assume "x \<in> proc1 R \<alpha> ` P"
+    then obtain p where p: "p \<in> P" "x = proc1 R \<alpha> p" by blast
     thus ?thesis
     proof (cases "ord (inst \<alpha>) p")
       case True
-      thus ?thesis using p ord by auto
+      thus ?thesis using p ord by (auto simp: proc1_def)
     next
       case False
-      thus ?thesis using p ooo by auto
+      thus ?thesis using p ooo by (auto simp: proc1_def)
     qed
   qed
-qed
+qed*)
 
-lemma upd_exec'':
-  assumes "lexecute c r \<alpha> c'"
-  assumes "\<forall>p \<in> upd2 R c P. inv p"
-  shows "\<forall>p \<in> upd2 R c' P. inv p"
+(*
+This isn't quite right, as this relation won't be preserved across
+earlier actions.
+
+*)
+
+definition set_ord (infix "\<lhd>" 60)
+  where "set_ord P' P \<equiv> \<forall>p' \<in> P'. \<exists>p \<in> P. p' \<prec> p"
+
+definition ignore_deps ("_ \<prec>_,_,_\<prec> _" 60)
+  where "ignore_deps P \<alpha> r R P' \<equiv> rif r P \<lhd> rif r (rif\<^sub>i \<alpha> P')"
+
+lemma ignore_deps_pres:
+  assumes "reorder_inst \<alpha>' \<beta> (fwd_com \<alpha> r)"
+  shows "P \<prec>\<alpha>,r,R\<prec> Q \<Longrightarrow> rif\<^sub>i \<beta> P \<prec>\<alpha>,Basic \<beta>;;r,R\<prec> rif\<^sub>i \<beta> Q"
+  unfolding ignore_deps_def proc\<^sub>i_def set_ord_def rif\<^sub>i_def by auto
+
+lemma rif_transitive:
+  assumes "reorder_com \<alpha>' r' (fwd_com \<alpha> r)"
+  shows "P \<prec>\<alpha>,r,R\<prec> Q \<Longrightarrow> rif r' P \<prec>\<alpha>,r';;r,R\<prec> rif r' Q"
   using assms
+proof (induct r' arbitrary: r \<alpha>' \<alpha> P Q)
+  case Nil
+  then show ?case by (auto simp: ignore_deps_def)
+next
+  case (Basic \<beta>)
+  thus ?case using ignore_deps_pres apply simp sorry
+next
+  case (Seq r\<^sub>1 r\<^sub>2)
+  obtain \<alpha>'' where r: "reorder_com \<alpha>'' r\<^sub>2 (fwd_com \<alpha> r)" "reorder_com \<alpha>' r\<^sub>1 (fwd_com \<alpha> (r\<^sub>2 ;; r))"
+    using Seq by auto
+  have s: "SimAsm_Inter.rif r\<^sub>2 P \<prec>\<alpha>,r\<^sub>2 ;; r,R\<prec> SimAsm_Inter.rif r\<^sub>2 Q"
+    using Seq(2)[OF Seq(3) r(1)] by auto
+  show ?case using Seq(1)[OF s r(2)] 
+    unfolding ignore_deps_def by auto
+qed auto
+
+lemma rif_lexecute:
+  assumes "lexecute c r \<alpha> c'"
+  shows "\<exists>c\<^sub>2. rif c P = rif ((r ;; Basic \<alpha>) ;; c\<^sub>2) P \<and> rif c' P = rif (r ;; c\<^sub>2) P"
+using assms
 proof (induct arbitrary: P)
   case (act \<alpha>)
-  then show ?case
-  proof (clarsimp)
-    fix x assume a: "x \<in> P"
-    show "point.inv x" 
-    proof (cases "ord (inst \<alpha>) x")
-      case True
-      hence "stren (inst \<alpha>) x \<in> upd\<^sub>a R \<alpha> P" using upd\<^sub>aI1[OF a, of \<alpha>] by simp
-      then show ?thesis using act by auto
-    next
-      case False
-      hence "(weaken (inst \<alpha>) x)\<lparr>inv := inv x \<and> chk R \<alpha> x\<rparr> \<in> upd\<^sub>a R \<alpha> P"
-        using upd\<^sub>aI1[OF a, of \<alpha>] by simp
-      then show ?thesis using act by auto
-    qed
-  qed
+  have a: "rif\<^sub>i \<alpha> P = rif\<^sub>i \<alpha> (SimAsm_Inter.rif Nil P)" "P = rif Nil P" by auto
+  show ?case apply auto using a by blast
 next
   case (ino c\<^sub>1 r \<alpha> c\<^sub>1' c\<^sub>2)
-  then show ?case by auto
+  then obtain c where 
+    "rif (c\<^sub>1 ;; c\<^sub>2) P = rif ((r ;; Basic \<alpha>) ;; c ;; c\<^sub>2) P" 
+    "rif (c\<^sub>1' ;; c\<^sub>2) P = rif (r ;; c ;; c\<^sub>2) P"
+    by force
+  then show ?case by blast
 next
   case (ooo c\<^sub>1 r \<alpha> c\<^sub>1' \<alpha>' c\<^sub>2)
-  then show ?case apply auto sorry
+  then obtain c where "rif c\<^sub>1 P = rif ((r ;; Basic \<alpha>) ;; c) P" "rif c\<^sub>1' P = rif (r ;; c) P" 
+    by force
+  then show ?case by auto
 qed
 
-theorem try_again:
+theorem rif_sound_helper:
   assumes "reorder_trace t c" "local c"
-  assumes "\<forall>p \<in> upd2 R c P. inv p"
+  assumes "\<forall>p \<in> rif c P. inv p"
   shows "\<forall>(r,\<alpha>) \<in> set t. inter\<^sub>c (step\<^sub>t R) (step G) r \<alpha>"
   using assms
 proof (induct)
@@ -416,113 +609,272 @@ next
   then show ?case using upd_rw[OF 2(1)] local_silent by blast
 next
   case (3 c r \<alpha> c' t)
-  then show ?case using upd_exec[OF 3(1,5), of G] local_execute[OF 3(1,4)] by auto
+  obtain c\<^sub>2 where "rif c P = rif ((r ;; Basic \<alpha>) ;; c\<^sub>2) P" "rif c' P = rif (r ;; c\<^sub>2) P"
+    using rif_lexecute 3 by metis
+  then show ?case using  local_execute[OF 3(1,4)] by auto
 qed
-
-theorem upd_correct:
-  assumes "\<forall>p \<in> upd2 R (lift\<^sub>c c) P. inv p"
-  shows "rif (step\<^sub>t R) (step G) (lift\<^sub>c c)"
-  using assms unfolding rif_def
-proof (intro impI allI ballI, goal_cases)
-  case (1 t x)
-  have l: "local (lift\<^sub>c c)" by blast
-  then show ?case using try_again[OF 1(2) l 1(1)] 1(3) by auto
-qed
-
-fun com_rgs
-  where 
-    "com_rgs (Basic a) = priv (rd (fst (tag a)))" |
-    "com_rgs (com.Seq c\<^sub>1 c\<^sub>2) = com_rgs c\<^sub>1 \<union> com_rgs c\<^sub>2" |
-    "com_rgs (Choice c\<^sub>1 c\<^sub>2) = com_rgs c\<^sub>1 \<union> com_rgs c\<^sub>2" |
-    "com_rgs (Loop c) = com_rgs c" |
-    "com_rgs _ = {}"
-
-fun com_glbs
-  where 
-    "com_glbs (Basic a) = shr (rd (fst (tag a))) \<union> shr (wr (fst (tag a)))" |
-    "com_glbs (com.Seq c\<^sub>1 c\<^sub>2) = com_glbs c\<^sub>1 \<union> com_glbs c\<^sub>2" |
-    "com_glbs (Choice c\<^sub>1 c\<^sub>2) = com_glbs c\<^sub>1 \<union> com_glbs c\<^sub>2" |
-    "com_glbs (Loop c) = com_glbs c" |
-    "com_glbs _ = {}"
-
-
-(*
-
-fun prog_rgs
-  where 
-    "prog_rgs Skip = {}" |
-    "prog_rgs (Op v e f) = priv (rd e)" |
-    "prog_rgs (Seq c\<^sub>1 c\<^sub>2) = prog_rgs c\<^sub>1 \<union> prog_rgs c\<^sub>2" |
-    "prog_rgs (If b c\<^sub>1 c\<^sub>2) = priv (deps\<^sub>B b) \<union> prog_rgs c\<^sub>1 \<union> prog_rgs c\<^sub>2" |
-    "prog_rgs (While b I c) = priv (deps\<^sub>B b) \<union> prog_rgs c" |
-    "prog_rgs (DoWhile I c b) = priv (deps\<^sub>B b) \<union> prog_rgs c"
-
-fun prog_glbs
-  where 
-    "prog_glbs Skip = {}" |
-    "prog_glbs (Op v e f) = shr (rd e) \<union> shr (wr e)" |
-    "prog_glbs (Seq c\<^sub>1 c\<^sub>2) = prog_glbs c\<^sub>1 \<union> prog_glbs c\<^sub>2" |
-    "prog_glbs (If b c\<^sub>1 c\<^sub>2) = shr (deps\<^sub>B b) \<union> prog_glbs c\<^sub>1 \<union> prog_glbs c\<^sub>2" |
-    "prog_glbs (While b I c) = shr (deps\<^sub>B b) \<union> prog_glbs c" |
-    "prog_glbs (DoWhile I c b) = shr (deps\<^sub>B b) \<union> prog_glbs c"
-
-fun prog_ops
-  where 
-    "prog_ops Skip = {}" |
-    "prog_ops (Op v e f) = { (\<lfloor>v,e,f\<rfloor>) }" |
-    "prog_ops (Seq c\<^sub>1 c\<^sub>2) = prog_ops c\<^sub>1 \<union> prog_ops c\<^sub>2" |
-    "prog_ops (If b c\<^sub>1 c\<^sub>2) = { (\<lfloor>cmp b\<rfloor>) } \<union> prog_ops c\<^sub>1 \<union> prog_ops c\<^sub>2" |
-    "prog_ops (While b I c) = { (\<lfloor>cmp b\<rfloor>) } \<union> prog_ops c" |
-    "prog_ops (DoWhile I c b) = { (\<lfloor>cmp b\<rfloor>) } \<union> prog_ops c"
 *)
 
-fun glbs
+fun expand :: "(nat, nat) com \<Rightarrow> ('v,'g,'r,'a) enuml \<Rightarrow> (('v,'g,'r,'a) auxop, ('v,'g,'r,'a) state) com"
   where
-    "glbs p = rds p \<union> wrs p"
+    "expand Nil l = Nil" |
+    "expand (Basic a) l = (case l ! tag a of (v,\<alpha>,f) \<Rightarrow> Basic (\<lfloor>v,\<alpha>,f\<rfloor>))" |
+    "expand (com.Seq c\<^sub>1 c\<^sub>2) l = com.Seq (expand c\<^sub>1 l) (expand c\<^sub>2 l)" |
+    "expand (Choice c\<^sub>1 c\<^sub>2) l = Choice (expand c\<^sub>1 l) (expand c\<^sub>2 l)" |
+    "expand (Loop c\<^sub>1) l = Loop (expand c\<^sub>1 l)" |
+    "expand (Parallel c\<^sub>1 c\<^sub>2) l = Parallel (expand c\<^sub>1 l) (expand c\<^sub>2 l)" |
+    "expand (Thread c\<^sub>1) l = Thread (expand c\<^sub>1 l)"
 
-definition all_points
-  where "all_points rs gs os \<equiv> {p. op p \<in> os \<and> rgs p \<subseteq> rs \<and> wrs p \<subseteq> gs \<and> rds p \<subseteq> gs}"
+lemma expand_seqE [elim!]:
+  assumes "expand n l = c\<^sub>1 ;; c\<^sub>2"
+  obtains n\<^sub>1 n\<^sub>2 where "expand n\<^sub>1 l = c\<^sub>1" "expand n\<^sub>2 l = c\<^sub>2" "n = n\<^sub>1 ;; n\<^sub>2"
+  using assms by (cases "(n,l)" rule: expand.cases) (auto split: prod.splits)
 
-lemma bound:
-  "upd2 R c P \<subseteq> all_points (com_rgs c \<union> \<Union> (rgs ` P)) (com_glbs c \<union> \<Union> (glbs ` P)) (basics c \<union> (op ` P))"
-  sorry
+lemma expand_seqE' [elim!]:
+  assumes "c\<^sub>1 ;; c\<^sub>2  = expand n l"
+  obtains n\<^sub>1 n\<^sub>2 where "expand n\<^sub>1 l = c\<^sub>1" "expand n\<^sub>2 l = c\<^sub>2" "n = n\<^sub>1 ;; n\<^sub>2"
+  using assms by (cases "(n,l)" rule: expand.cases) (auto split: prod.splits)
 
-lemma finite_all_points:
-  "finite rs \<Longrightarrow> finite gs \<Longrightarrow> finite os \<Longrightarrow> finite (all_points rs gs os)"
-  unfolding all_points_def sorry
+lemma expand_nilE [elim!]:
+  assumes "expand n l = com.Nil"
+  obtains "n = com.Nil"
+  using assms by (cases "(n,l)" rule: expand.cases) (auto split: prod.splits)
 
-lemma upd_While:
-  fixes b c P R
-  assumes "finite P"
-  defines "f == (\<lambda>Y. (P \<union> upd2 R c Y))"
-  shows "upd2 R (Loop c) P = while (\<lambda>Y. f Y \<noteq> Y) f {}" (is "_ = ?r")
-proof -
-  let ?V = "all_points (com_rgs c \<union> \<Union> (rgs ` P)) (com_glbs c \<union> \<Union> (glbs ` P)) (basics c \<union> (op ` P))"
-  have "lfp f = ?r"
-  proof(rule lfp_while[where C = "?V"])
-    show "mono f" using f_def mono_union_upd2 by blast
-  next
-    fix Y show "Y \<subseteq> ?V \<Longrightarrow> f Y \<subseteq> ?V"
-      unfolding f_def using bound[of R c] by blast
-  next
-    show "finite ?V" using \<open>finite P\<close>
-      apply (intro finite_all_points)
-      by simp
-  qed
-  thus ?thesis by (simp add: f_def)
+lemma expand_nilE' [elim!]:
+  assumes "com.Nil = expand n l"
+  obtains "n = com.Nil"
+  using assms by (cases "(n,l)" rule: expand.cases) (auto split: prod.splits)
+
+lemma expand_choiceE [elim!]:
+  assumes "expand n l = Choice c\<^sub>1 c\<^sub>2"
+  obtains n\<^sub>1 n\<^sub>2 where "expand n\<^sub>1 l = c\<^sub>1" "expand n\<^sub>2 l = c\<^sub>2" "n = Choice n\<^sub>1 n\<^sub>2"
+  using assms by (cases "(n,l)" rule: expand.cases) (auto split: prod.splits)
+
+lemma expand_choiceE' [elim!]:
+  assumes "Choice c\<^sub>1 c\<^sub>2 = expand n l"
+  obtains n\<^sub>1 n\<^sub>2 where "expand n\<^sub>1 l = c\<^sub>1" "expand n\<^sub>2 l = c\<^sub>2" "n = Choice n\<^sub>1 n\<^sub>2"
+  using assms by (cases "(n,l)" rule: expand.cases) (auto split: prod.splits)
+
+lemma expand_loopE' [elim!]:
+  assumes "Loop c\<^sub>1 = expand n l"
+  obtains n\<^sub>1 where "expand n\<^sub>1 l = c\<^sub>1" "n = Loop n\<^sub>1"
+  using assms by (cases "(n,l)" rule: expand.cases) (auto split: prod.splits)
+
+lemma expand_basicE' [elim!]:
+  assumes "Basic b = expand n l"
+  obtains a v \<alpha> f where " l ! tag a = (v,\<alpha>,f)" "n = Basic a" "b = (\<lfloor>v,\<alpha>,f\<rfloor>)"
+  using assms by (cases "(n,l)" rule: expand.cases) (auto split: prod.splits)
+
+lemma rif_sound_sil:
+  assumes "c \<leadsto> c'" "local c" "c = expand n l"
+  obtains n' where "rif n (map (fst o snd) l) P \<supseteq> rif n' (map (fst o snd) l) P" "expand n' l = c'"
+  using assms
+proof (induct arbitrary: n P)
+  case (seq1 c\<^sub>1 c\<^sub>1' c\<^sub>2)
+  then obtain n\<^sub>1 n\<^sub>2 where n: "local c\<^sub>1" "c\<^sub>1 = expand n\<^sub>1 l" "expand n\<^sub>2 l = c\<^sub>2" "n = n\<^sub>1 ;; n\<^sub>2" by auto
+  show ?case 
+    apply (rule seq1(2)[OF _ n(1,2)])
+    apply (rule seq1(3)[of "n' ;; n\<^sub>2" for n'])
+    using n(3,4) by auto
+next
+  case (seq2 c\<^sub>2 c\<^sub>2' c\<^sub>1)
+  then obtain n\<^sub>1 n\<^sub>2 where n: "local c\<^sub>2" "c\<^sub>2 = expand n\<^sub>2 l" "c\<^sub>1 = expand n\<^sub>1 l" "n = n\<^sub>1 ;; n\<^sub>2" by auto
+  show ?case
+    apply (rule seq2(2)[OF _ n(1,2)])
+    apply (rule seq2(3)[of "n\<^sub>1 ;; n'" for n'])
+    using n apply auto 
+    using mono_rif[of n\<^sub>1 "map (\<lambda>a. fst (snd a)) l"] apply (drule monoD)
+    by auto
+next
+  case (seqE1 c\<^sub>1)
+  then obtain n\<^sub>1 where n:  "c\<^sub>1 = expand n\<^sub>1 l" "n = Nil ;; n\<^sub>1" by auto
+  then show ?case using seqE1(1)[of n\<^sub>1] by auto
+next
+  case (seqE2 c\<^sub>1)
+  then obtain n\<^sub>1 where n: "c\<^sub>1 = expand n\<^sub>1 l" "n = n\<^sub>1 ;; Nil" by auto
+  then show ?case using seqE2(1)[of n\<^sub>1] by auto
+next
+  case (left c\<^sub>1 c\<^sub>2)
+  then obtain n\<^sub>1 n\<^sub>2 where n: "local c\<^sub>1" "c\<^sub>1 = expand n\<^sub>1 l" "expand n\<^sub>2 l = c\<^sub>2" "n = Choice n\<^sub>1 n\<^sub>2" by auto
+  then show ?case using left(1)[of n\<^sub>1] by auto
+next
+  case (right c\<^sub>1 c\<^sub>2)
+  then obtain n\<^sub>1 n\<^sub>2 where n: "local c\<^sub>1" "c\<^sub>1 = expand n\<^sub>1 l" "expand n\<^sub>2 l = c\<^sub>2" "n = Choice n\<^sub>1 n\<^sub>2" by auto
+  then show ?case using right(1)[of n\<^sub>2] by auto
+next
+  case (loop1 c)
+  then obtain n\<^sub>1 where n: "n = Loop n\<^sub>1" by auto
+  thus ?case using loop1(1)[of "Nil"] lfp_unfold mono_union_rif by (auto simp: rif.simps(3))
+next
+  case (loop2 c)
+  then obtain n\<^sub>1 where n: "expand n\<^sub>1 l = c" "n = Loop n\<^sub>1" by auto
+  then show ?case using loop2(1)[of "n\<^sub>1 ;; n"] apply auto unfolding rif.simps
+    using lfp_fn[OF mono_rif] by blast
+qed (unfold local.simps; simp)+
+
+lemma rif_sound_exec:
+  assumes "lexecute c r \<alpha> c'" "local c" "c = expand n l"
+  obtains n' where "rif n (map (fst o snd) l) P \<supseteq> rif n' (map (fst o snd) l) P" "expand n' l = c'"
+  using assms
+proof (induct arbitrary: n P)
+  case (act \<alpha>)
+  then show ?case sorry
+next
+  case (ino c\<^sub>1 r \<alpha> c\<^sub>1' c\<^sub>2)
+  then show ?case sorry
+next
+  case (ooo c\<^sub>1 r \<alpha> c\<^sub>1' \<alpha>' c\<^sub>2)
+  then show ?case sorry
 qed
 
-lemma upd_While_let: "finite X \<Longrightarrow> upd2 R (Loop c) X =
-  (let f = (\<lambda>Y. X \<union> upd2 R c Y)
-   in while (\<lambda>Y. f Y \<noteq> Y) f {})"
-by(simp add: upd_While)
+lemma rif_lexecute:
+  assumes "lexecute c r \<alpha> c'" "expand n l = c" 
+  obtains c\<^sub>2 n' where "rif n (map (fst o snd) l) P = rif n' (map (fst o snd) l) P" "expand n' l = ((r ;; Basic \<alpha>) ;; c\<^sub>2)"
+using assms
+proof (induct arbitrary: P n)
+  case (act \<alpha>)
+  show ?case using act(1)[of "(Nil ;; n) ;; Nil" Nil] act(2) by auto
+next
+  case (ino c\<^sub>1 r \<alpha> c\<^sub>1' c\<^sub>2)
+  obtain n\<^sub>1 n\<^sub>2 where n: "expand n\<^sub>1 l = c\<^sub>1" "expand n\<^sub>2 l = c\<^sub>2" "n = n\<^sub>1 ;; n\<^sub>2" using ino(4) by auto
+  show ?case
+  proof (rule ino(2)[OF _ n(1), of "rif n\<^sub>2 (map (fst \<circ> snd) l) P"], goal_cases)
+    case (1 n' c\<^sub>2')
+    then obtain n\<^sub>1' n\<^sub>2' where "expand n\<^sub>1' l = r ;; Basic \<alpha>" "expand n\<^sub>2' l = c\<^sub>2'" "n' = n\<^sub>1' ;; n\<^sub>2'"
+      by force
+    thus ?case 
+      using 1(1) n(2) ino(3)[of "n\<^sub>1' ;; (n\<^sub>2' ;; n\<^sub>2)" "c\<^sub>2' ;; c\<^sub>2"] 
+      by (auto simp: n(3) o_def) 
+  qed
+next
+  case (ooo c\<^sub>2 r \<alpha> c\<^sub>1' \<alpha>' c\<^sub>1)
+  then obtain n\<^sub>1 n\<^sub>2 where n: "expand n\<^sub>1 l = c\<^sub>1" "expand n\<^sub>2 l = c\<^sub>2" "n = n\<^sub>1 ;; n\<^sub>2" by auto
+  show ?case
+  proof (rule ooo(2)[OF _ n(2), of P], goal_cases)
+    case (1 n' c\<^sub>2')
+    then obtain n\<^sub>1' n\<^sub>2' where n': "expand n\<^sub>1' l = r ;; Basic \<alpha>" "expand n\<^sub>2' l = c\<^sub>2'" "n' = n\<^sub>1' ;; n\<^sub>2'"
+      by force
+    then obtain n\<^sub>1'' n\<^sub>2'' where n'': "expand n\<^sub>1'' l = r" "expand n\<^sub>2'' l = Basic \<alpha>" "n\<^sub>1' = n\<^sub>1'' ;; n\<^sub>2''"
+      by force
+    then show ?case
+      using 1(1) n(1,2) n'(1,2) ooo(4)[of "((n\<^sub>1 ;; n\<^sub>1'') ;; n\<^sub>2'') ;; n\<^sub>2'" c\<^sub>2']
+      by (auto simp: n(3) n'(3))
+  qed
+qed
 
-lemma upd_While_set: "upd2 R (Loop c) (set xs) =
-  (let f = (\<lambda>Y. set xs \<union> upd2 R c Y)
-   in while (\<lambda>Y. f Y \<noteq> Y) f {})"
-by(rule upd_While_let, simp)
+lemma rif_lexecute':
+  assumes "lexecute c r \<alpha> c'" "expand n l = c" 
+  obtains c\<^sub>2 n' n'' n''' where 
+    "rif n (map (fst o snd) l) P = rif n' (map (fst o snd) l) P" 
+    "expand n' l = ((r ;; Basic \<alpha>) ;; c\<^sub>2)"
+    "expand n'' l = c'"
+    "expand n''' l = (r ;; c\<^sub>2)"
+    "rif n'' (map (fst o snd) l) P = rif n''' (map (fst o snd) l) P" 
+using assms
+proof (induct arbitrary: P n)
+  case (act \<alpha>)
+  show ?case using act(1)[of "(Nil ;; n) ;; Nil" Nil Nil "Nil ;; Nil"] act(2) by auto
+next
+  case (ino c\<^sub>1 r \<alpha> c\<^sub>1' c\<^sub>2)
+  obtain n\<^sub>1 n\<^sub>2 where n: "expand n\<^sub>1 l = c\<^sub>1" "expand n\<^sub>2 l = c\<^sub>2" "n = n\<^sub>1 ;; n\<^sub>2" using ino(4) by auto
+  show ?case
+  proof (rule ino(2)[OF _ n(1), of "rif n\<^sub>2 (map (fst \<circ> snd) l) P"], goal_cases)
+    case (1 n' c\<^sub>2' n'' n''')
+    then obtain n\<^sub>1' n\<^sub>2' where n': "expand n\<^sub>1' l = r ;; Basic \<alpha>" "expand n\<^sub>2' l = c\<^sub>2'" "n' = n\<^sub>1' ;; n\<^sub>2'"
+      by force
+    then obtain n\<^sub>1'' n\<^sub>2'' where n'': "expand n\<^sub>1'' l = r" "expand n\<^sub>2'' l = Basic \<alpha>" "n\<^sub>1' = n\<^sub>1'' ;; n\<^sub>2''"
+      by force
+    thus ?case 
+      using n' 1(1,3,4,5) n(2) ino(3)[of "n\<^sub>1' ;; (n\<^sub>2' ;; n\<^sub>2)" "c\<^sub>2' ;; c\<^sub>2" "n'' ;; n\<^sub>2" "n\<^sub>1'' ;; n\<^sub>2' ;; n\<^sub>2"] 
+      by (auto simp: n(3) o_def) 
+  qed
+next
+  case (ooo c\<^sub>2 r \<alpha> c\<^sub>1' \<alpha>' c\<^sub>1)
+  then obtain n\<^sub>1 n\<^sub>2 where n: "expand n\<^sub>1 l = c\<^sub>1" "expand n\<^sub>2 l = c\<^sub>2" "n = n\<^sub>1 ;; n\<^sub>2" by auto
+  show ?case
+  proof (rule ooo(2)[OF _ n(2), of P], goal_cases)
+    case (1 n' c\<^sub>2')
+    then obtain n\<^sub>1' n\<^sub>2' where n': "expand n\<^sub>1' l = r ;; Basic \<alpha>" "expand n\<^sub>2' l = c\<^sub>2'" "n' = n\<^sub>1' ;; n\<^sub>2'"
+      by force
+    then obtain n\<^sub>1'' n\<^sub>2'' where n'': "expand n\<^sub>1'' l = r" "expand n\<^sub>2'' l = Basic \<alpha>" "n\<^sub>1' = n\<^sub>1'' ;; n\<^sub>2''"
+      by force
+    then show ?case
+      using 1(1) n(1,2) n'(1,2) ooo(4)[of "((n\<^sub>1 ;; n\<^sub>1'') ;; n\<^sub>2'') ;; n\<^sub>2'" c\<^sub>2']
+      by (auto simp: n(3) n'(3))
+  qed
+qed
 
-lemmas [code] = upd2.simps(1,2,4,5) upd_While_set
+lemma upd_exec':
+  assumes "lexecute c r \<alpha> c'" "expand n l = c"
+  assumes "checks l (rif n (map (fst o snd) l) P) R"
+  shows "inter\<^sub>c (step\<^sub>t R) (step G) r \<alpha>"
+  using assms
+proof (induct arbitrary: n P)
+  case (act \<alpha>)
+  then show ?case by auto
+next
+  case (ino c\<^sub>1 r \<alpha> c\<^sub>1' c\<^sub>2)
+  then show ?case by auto
+next
+  case (ooo c\<^sub>2 r \<alpha> c\<^sub>1' \<alpha>' c\<^sub>1)
+  then obtain n\<^sub>1 n\<^sub>2 where n: "expand n\<^sub>1 l = c\<^sub>1" "expand n\<^sub>2 l = c\<^sub>2" "n = n\<^sub>1 ;; n\<^sub>2" by auto
+  hence "inter\<^sub>c (step\<^sub>t R) (step G) r \<alpha>" using ooo(5) ooo(2)[OF n(2), of P]
+    unfolding n(3)
+    sorry
+  then show ?case sorry
 
+  then obtain p where p: "p \<in> rif c\<^sub>1 P" "op p = fwd_com \<alpha> r" "point_cmp p (gen (fwd_com \<alpha> r))"
+    using execute_act by blast
+  have r: "reorder_com \<alpha>' (c\<^sub>2) (fwd_com \<alpha> r)" using ooo by auto
+  have f: "fwd_com \<alpha> r =  (op p) " using p by auto
+  have "inter\<^sub>c (step\<^sub>t R) (step G) r \<alpha>" using ooo rif_preserve_inv by force
+  thus ?case using upd_po[OF r p(1,3) f] ooo(4) by auto
+qed  
+
+lemma [simp]:
+  "tag (\<lfloor>v,\<alpha>,f\<rfloor>) = (\<alpha>,f)"
+  by (auto simp: liftg_def)
+
+lemma
+  assumes "reorder_com \<alpha>' r \<alpha>"
+  assumes "r = expand n l" "\<forall>a \<in> basics n. tag a < length l" 
+  assumes "Basic \<alpha> = expand (Basic a) l" "tag a < length l"
+  assumes "checks l (rif (n ;; Basic a)  (map (fst o snd) l) P) R"
+  shows "inter\<^sub>c (step\<^sub>t R) (step G) r \<alpha>"
+  using assms
+proof (induct arbitrary: n a rule: reorder_com.induct )
+  case (2 \<alpha>' \<beta> \<alpha>)
+  then show ?case
+    apply (auto split: prod.splits)
+    sorry
+next
+  case (3 \<alpha>' c\<^sub>1 c\<^sub>2 \<alpha>)
+  then show ?case sorry
+qed (unfold reorder_com.simps, auto)
+
+theorem rif_sound:
+  assumes "reorder_trace t c" "local c"
+  assumes "expand n l = c"
+  assumes "checks l (rif n (map (fst o snd) l) {}) R"
+  shows "\<forall>(r,\<alpha>) \<in> set t. inter\<^sub>c (step\<^sub>t R) (step G) r \<alpha>"
+  using assms
+proof (induct arbitrary: n)
+  case (1 c)
+  then show ?case by auto
+next
+  case (2 c c' t)
+  then obtain n' where "rif n (map (fst o snd) l) {} \<supseteq> rif n' (map (fst o snd) l) {}" "expand n' l = c'"
+    using rif_sound_sil by metis
+  moreover have "local c'" using 2 local_silent by auto
+  ultimately show ?case using 2 unfolding checks_def by blast
+next
+  case (3 c r \<alpha> c' t)
+  then obtain c\<^sub>2 n' where 
+      "rif n (map (fst o snd) l) {} = rif n' (map (fst o snd) l) {}" 
+      "expand n' l = ((r ;; Basic \<alpha>) ;; c\<^sub>2)"
+    using rif_lexecute by metis
+
+  then show ?case sorry
+qed
 
 end
