SimAsm/SimAsm_Inter_Exec.thy
@@ -1,0 +1,433 @@
+theory SimAsm_Inter_Exec
+  imports SimAsm_Inter "HOL-Library.While_Combinator" "HOL-Eisbach.Eisbach"
+begin
+
+text \<open>
+Theorems to demonstrate termination of the SimAsm_Inter analysis 
+and demonstrate its conversion to executable definitions.
+\<close>
+
+section \<open>Termination Proof\<close>
+
+abbreviation vars
+  where "vars p \<equiv> (rds p |\<union>| wrs p)"
+
+definition nmax
+  where "nmax V \<equiv> if V = {||} then 0 else fMax V"
+
+definition pmax
+  where "pmax p \<equiv> max (id p) (nmax (pairs p))"
+
+definition Pmax
+  where "Pmax P \<equiv> if P = {} then 0 else Max (pmax ` P)"
+
+definition varsL
+  where "varsL l = Sup ((\<lambda>p. fwr p |\<union>| frd p) ` (set l))"
+
+definition all_points
+  where "all_points vs i \<equiv> {p. vars p |\<subseteq>| vs \<and> id p \<le> i \<and> nmax (pairs p) \<le> i}"
+
+lemma finite_all_points [intro]:
+  "finite (all_points vs i :: ('a, 'b) point set)"
+proof -
+  let ?f = "\<lambda>d w r b p. \<lparr>id = d, wrs = w, rds = r, bar = b, pairs = p\<rparr>"
+  have a: "finite {w. w |\<subseteq>| vs}"
+  proof -
+    have "finite (Abs_fset ` {w. w \<subseteq> fset vs})" by simp
+    moreover have "{w. w |\<subseteq>| vs} \<subseteq> Abs_fset ` {w. w \<subseteq> fset vs}"
+      by (auto simp: fset_inverse less_eq_fset.rep_eq rev_image_eqI)
+    ultimately show ?thesis by (meson finite_subset)
+  qed
+  have b: "finite {p. nmax p \<le> i}"
+  proof -
+    have "finite {p. p \<subseteq> {j. j \<le> i}}" by blast
+    hence f: "finite {p. finite p \<and> Max p \<le> i}"
+      by (rule rev_finite_subset; insert Max.boundedE; auto)
+    hence "finite (insert {||} (Abs_fset ` {p. finite p \<and> Max p \<le> i}))" 
+      by blast
+    thus ?thesis
+      apply (rule rev_finite_subset)
+      apply (auto simp: nmax_def)
+      by (metis (no_types, lifting) fMax.F.rep_eq finite_fset fset_inverse image_iff mem_Collect_eq)
+  qed
+  have c: "finite {?f d w r b p | d w r b p. w |\<subseteq>| vs \<and> r |\<subseteq>| vs \<and> d \<le> i \<and> nmax p \<le> i}"
+    using a b finite_subset[where 
+        A="{?f d w r b p | d w r b p. w |\<subseteq>| vs \<and> r |\<subseteq>| vs \<and> d \<le> i \<and> nmax p \<le> i}" and 
+        B="\<Union>d \<in> {d. d \<le> i}. \<Union>w \<in> {w. w |\<subseteq>| vs}. \<Union>r \<in> {r. r |\<subseteq>| vs}. \<Union>b \<in> UNIV. \<Union>p \<in> {p. nmax p \<le> i}. {?f d w r b p}"]
+    by fastforce
+  have d: "all_points vs i \<subseteq> {?f d w r b p | d w r b p. w |\<subseteq>| vs \<and> r |\<subseteq>| vs \<and> d \<le> i \<and> nmax p \<le> i}"
+    unfolding all_points_def
+    by auto (metis point.cases point.select_convs(1,2,3,5))
+  show "finite (all_points vs i :: ('a, 'b) point set)"
+    using finite_subset[OF d c] .
+qed
+
+lemma all_points_rel:
+  "P |\<subseteq>| P' \<Longrightarrow> i \<le> i' \<Longrightarrow> all_points P i \<subseteq> all_points P' i'"
+  unfolding all_points_def by auto
+
+lemma max_fg:
+  assumes "finite P" "\<forall>p. f p \<le> g p"
+  shows "Max (f ` P) \<le> Max (g ` P)"
+  using assms 
+  by (smt Max_ge_iff Max_in finite_imageI imageE image_eqI image_is_empty order_refl) 
+
+lemma Max_max :
+  "finite V \<Longrightarrow> Max ((\<lambda>p. max (f p) (g p)) ` V) = max (Max (f ` V)) (Max (g ` V))" (is "finite V \<Longrightarrow> ?L = ?R")
+proof -
+  assume a: "finite V"
+  have "?L \<ge> ?R"
+  proof -
+    have "Max (f ` V) \<le> ?L" using a by (rule max_fg) auto
+    moreover have "Max (g ` V) \<le> ?L" using a by (rule max_fg) auto
+    ultimately show "?L \<ge> ?R" by auto
+  qed
+  moreover have "?R \<ge> ?L"
+  proof (cases "Max (f ` V) \<ge> Max (g ` V)")
+    case True
+    hence "max (Max (f ` V)) (Max (g ` V)) = Max (f ` V)" using max_absorb1 by blast
+    moreover have "(MAX p\<in>V. max (f p) (g p)) \<le> (Max (f ` V))" using a
+      by (smt Max_ge Max_in calculation dual_order.trans finite_imageI image_iff image_is_empty max.absorb_iff1 max_def)
+    ultimately show ?thesis by auto
+  next
+    case False
+    hence "max (Max (f ` V)) (Max (g ` V)) = Max (g ` V)" using linear max_absorb2 by blast
+    moreover have "(MAX p\<in>V. max (f p) (g p)) \<le> (Max (g ` V))" using a
+      by (smt Max_ge Max_in calculation dual_order.trans finite_imageI image_iff image_is_empty max.absorb_iff1 max_def)
+    ultimately show ?thesis by auto
+  qed
+  ultimately show ?thesis using eq_iff by blast
+qed
+
+lemma set_all_points_bound:
+  "finite P \<Longrightarrow> P \<subseteq> all_points (Sup (vars ` P)) (Pmax P)"
+  unfolding all_points_def
+proof (clarsimp, intro conjI, goal_cases)
+  case (1 x)
+  hence "vars x |\<subseteq>| Sup (vars ` P)" 
+    by (meson finite_imageI image_iff le_cSup_finite)
+  then show ?case by blast
+next
+  case (2 x)
+  hence "vars x |\<subseteq>| Sup (vars ` P)" 
+    by (meson finite_imageI image_iff le_cSup_finite)
+  then show ?case by blast
+next
+  case (3 x)
+  hence "id x \<le> (MAX p\<in>P. id p)" by simp
+  also have "... \<le> (MAX p\<in>P. max (id p) (nmax (pairs p)))"
+    apply (rule max_fg)
+    using 3 by auto
+  also have "... \<le> Pmax P" using 3 by (auto simp: Pmax_def pmax_def)
+  finally show ?case .
+next
+  case (4 x)
+  hence "nmax (pairs x) \<le> (MAX p\<in>P. nmax (pairs p))" by simp
+  also have "... \<le> (MAX p\<in>P. max (id p) (nmax (pairs p)))"
+    apply (rule max_fg)
+    using 4 by auto
+  also have "... \<le> Pmax P" using 4 by (auto simp: Pmax_def pmax_def)
+  finally show ?case .
+qed
+
+lemma set_all_points_bound':
+  "finite P \<Longrightarrow> P \<subseteq> all_points (varsL l |\<union>| Sup (vars ` P)) (max (length l) (Pmax P))"
+  using set_all_points_bound all_points_rel
+  by (metis (mono_tags, lifting) subset_trans sup_ge2 sup_max)
+
+lemma fsubset_sup:
+  "\<forall>j \<in> Y. f j |\<subseteq>| X \<Longrightarrow> Sup (f ` Y) |\<subseteq>| X"
+proof -
+  assume "\<forall>j \<in> Y. f j |\<subseteq>| X"
+  hence "\<forall>j \<in> Y. fset (f j) \<subseteq> fset X" by (simp add: less_eq_fset.rep_eq)
+  hence "Sup ((fset o f) ` Y) \<subseteq> fset X" by auto
+  thus "Sup (f ` Y) |\<subseteq>| X" 
+    by (simp add: Sup_fset.rep_eq less_eq_fset.rep_eq) 
+qed
+
+lemma all_points_sub:
+  assumes "Y \<subseteq> (all_points vs i :: ('a, 'b) point set)"
+  shows "all_points (Sup (vars ` Y)) (Pmax Y) \<subseteq> all_points vs i"
+proof (rule all_points_rel)
+  have "\<forall>j \<in> pmax ` Y. j \<le> i"
+    using assms by (auto simp: all_points_def pmax_def)
+  moreover have "finite Y" using finite_subset[OF assms finite_all_points] .
+  ultimately show "Pmax Y \<le> i" unfolding Pmax_def by auto
+next
+  have "\<forall>j \<in> Y. vars j |\<subseteq>| vs" using assms by (auto simp: all_points_def)
+  thus "Sup (vars ` Y) |\<subseteq>| vs" using fsubset_sup by fast
+qed
+
+lemma all_points_rel_rev:
+  "all_points v i \<subseteq> (all_points v' i' :: ('a, 'b) point set) \<Longrightarrow> (v |\<subseteq>| v' \<and> i \<le> i')"
+proof (rule ccontr)
+  assume s: "all_points v i \<subseteq> (all_points v' i' :: ('a, 'b) point set)" "\<not> (v |\<subseteq>| v' \<and> i \<le> i')"
+  hence "\<not> v |\<subseteq>| v' \<or> i > i'" by auto
+  hence "\<lparr>id = i, wrs = v, rds = v, bar = True, pairs = {||}\<rparr> \<notin> all_points v' i'"
+    by (auto simp: all_points_def nmax_def)
+  moreover have "\<lparr>id = i, wrs = v, rds = v, bar = True, pairs = {||}\<rparr> \<in> all_points v i"
+    by (auto simp: all_points_def nmax_def)
+ ultimately show "False" using s(1) by auto
+qed
+
+lemma all_points_const:
+  assumes "all_points v i \<subseteq> (all_points v' i' :: ('a, 'b) point set)"
+  shows "all_points (c |\<union>| v) (max ic i) \<subseteq> all_points (c |\<union>| v') (max ic i')"
+proof -
+  have "v |\<subseteq>| v' \<and> i \<le> i'" using all_points_rel_rev[OF assms] by auto
+  thus ?thesis by (intro all_points_rel) auto
+qed
+
+lemma [simp]:
+  "Sup (vars ` (all_points vs i :: ('a, 'b) point set) ) = vs"
+proof -
+  let ?f = "\<lambda>d w r b p. \<lparr>id = d, wrs = w, rds = r, bar = b, pairs = p\<rparr>"
+  have a: "(all_points vs i :: ('a, 'b) point set) = {?f d w r b p | d w r b p. w |\<subseteq>| vs \<and> r |\<subseteq>| vs \<and> d \<le> i \<and> nmax p \<le> i}"
+    unfolding all_points_def apply auto 
+    by (metis (full_types) old.unit.exhaust point.surjective)
+
+  have "(vars ` (all_points vs i :: ('a, 'b) point set)) = {j. j |\<subseteq>| vs}"
+    apply (auto simp: a)
+    apply (subgoal_tac "?f i x x True {||} \<in> all_points vs i")
+    unfolding a
+    apply force
+    by (auto simp: nmax_def)
+  moreover have "Sup {j. j |\<subseteq>| vs} = vs"
+    by (metis cSup_eq_maximum mem_Collect_eq order_refl)
+  ultimately show ?thesis by metis
+qed
+
+lemma all_points_nil:
+  "(all_points vs i :: ('a, 'b) point set) \<noteq> {}"
+proof -
+  have a: "\<lparr>id = 0, wrs = {||}, rds = {||}, bar = True, pairs = {||}\<rparr> \<in> all_points vs i"
+    by (auto simp: all_points_def nmax_def)
+  show ?thesis apply (rule ccontr) apply simp using a by blast
+qed
+
+lemma [simp]:
+  "Pmax (all_points vs i :: ('a, 'b) point set) = i"
+proof -
+  let ?f = "\<lambda>d w r b p. \<lparr>id = d, wrs = w, rds = r, bar = b, pairs = p\<rparr>"
+  have a: "(all_points vs i :: ('a, 'b) point set) = {?f d w r b p | d w r b p. w |\<subseteq>| vs \<and> r |\<subseteq>| vs \<and> d \<le> i \<and> nmax p \<le> i}"
+    unfolding all_points_def apply auto 
+    by (metis (full_types) old.unit.exhaust point.surjective)
+
+  have "id ` (all_points vs i  :: ('a, 'b) point set) = {j. j \<le> i}" unfolding a
+     apply auto 
+    by (smt fsubsetI mem_Collect_eq nmax_def point.simps(1) rev_image_eqI zero_order(1)) 
+  moreover have b: "Max {j. j \<le> i} = i"
+    by (metis Max_ge Max_in antisym emptyE finite_Collect_le_nat mem_Collect_eq order_refl)
+  ultimately have c: "Max (id ` (all_points vs i  :: ('a, 'b) point set)) = i" by simp
+
+  have "(nmax o pairs) ` (all_points vs i  :: ('a, 'b) point set) = {j. j \<le> i}" unfolding a
+    apply auto
+    apply (subgoal_tac "?f i vs vs True {|x|} \<in> all_points vs i")
+    apply (metis (no_types, lifting) a fMax.singleton finsert_not_fempty nmax_def point.select_convs(5) rev_image_eqI)
+    unfolding a by (auto simp: nmax_def)
+  hence d: "Max ((nmax o pairs) ` (all_points vs i  :: ('a, 'b) point set)) = i" using b by simp
+
+  have "(MAX p\<in>(all_points vs i :: ('a, 'b) point set). max (point.id p) (nmax (pairs p))) = i"
+    using Max_max[OF finite_all_points, of id "nmax o pairs" vs i]
+    unfolding c d by auto
+  thus "Pmax (all_points vs i :: ('a, 'b) point set) = i"
+    unfolding Pmax_def pmax_def using all_points_nil
+    by auto
+qed
+
+lemma sup_in:
+  assumes "finite P" "y \<in> P" "x |\<in>| f y"
+  shows "x |\<in>| Sup (f ` P)"
+proof -
+  have "x \<in> fset (f y)" using assms(3) by (meson notin_fset)
+  hence a: "x \<in> Sup ((fset o f) ` P)" using assms(2) by auto
+  have f: "finite ((\<Union>a\<in>P. fset (f a)))" using assms(1) by simp
+  hence "Sup ((fset o f) ` P) =  fset (Sup (f ` P))" 
+    unfolding Sup_fset_def apply auto
+    using Abs_fset_inverse f apply blast
+    using Abs_fset_inverse f by blast  
+  thus ?thesis using a notin_fset by metis
+qed
+
+lemma sup_in_l:
+  assumes "i < length l" "x |\<in>| f (l ! i)"
+  shows "x |\<in>| Sup (f ` set l)"
+  using assms sup_in[of "set l" "l ! i" x f] by auto
+
+lemma [simp]:
+  "nmax (finsert a b) = max (a :: nat) (nmax b)"
+  unfolding nmax_def by auto
+
+lemma proc1_all_points:
+  "finite P \<Longrightarrow> xa \<in> P \<Longrightarrow> tag x < length l \<Longrightarrow>
+          proc1 (tag x) (l ! tag x) xa
+          \<in> all_points
+              (varsL l |\<union>| Sup (vars ` P))
+              (max (length l) (Pmax P))"
+  unfolding proc1_def
+  apply (subgoal_tac "xa \<in> all_points
+              (varsL l |\<union>| Sup (vars ` P))
+              (max (length l) (Pmax P))")
+  apply (auto simp: all_points_def varsL_def)
+  apply (rule sup_in_l; blast)+
+
+  apply (subgoal_tac "xb |\<in>| Sup (vars ` P)")
+  apply simp
+  apply (rule sup_in)
+  apply blast
+  apply blast
+  apply blast
+
+  apply (subgoal_tac "xb |\<in>| Sup (vars ` P)")
+  apply simp
+  apply (rule sup_in)
+  apply blast
+  apply blast
+  apply blast
+
+  unfolding Pmax_def pmax_def
+  apply (simp add: Max_max)
+  apply (metis Max.bounded_iff empty_iff finite_imageI image_eqI max.cobounded1 max.coboundedI2)
+  apply (simp add: Max_max)
+  by (meson Max_ge empty_iff finite_imageI imageI le_max_iff_disj)
+
+lemma gen_all_points:
+  "tag x < length l \<Longrightarrow>
+          gen (tag x) (l ! tag x)
+          \<in> all_points
+              (varsL l |\<union>| Sup (vars ` P))
+              (max (length l) (Pmax P))"
+  unfolding gen_def all_points_def nmax_def varsL_def
+  apply auto
+  apply (rule sup_in_l; blast)+
+  done
+
+lemma rif_bound:
+  "finite P \<Longrightarrow> rif c l P \<subseteq> (all_points (varsL l |\<union>| Sup (vars ` P)) (max (length l) (Pmax P)) :: ('a, 'b) point set)"
+proof (induct c arbitrary: P)
+  case Nil
+  then show ?case using set_all_points_bound' by auto
+next
+  case (Basic x)
+  thus ?case
+    apply (auto simp: rif\<^sub>i_def proc\<^sub>i_def)
+    apply (rule gen_all_points; auto)
+    apply (rule proc1_all_points; auto)
+    using set_all_points_bound' by auto
+next
+  case (Seq c1 c2)
+  let ?V="(all_points(varsL l |\<union>| Sup (vars ` P)) (max (length l) (Pmax P)) :: ('a, 'b) point set)"
+  have f: "finite ?V" using finite_all_points by auto
+  show ?case using Seq(1)[OF f] Seq(2)[OF Seq(3)] by simp (meson dual_order.trans monoD mono_rif)
+next
+  case (Choice c1 c2)
+  then show ?case by auto
+next
+  case (Loop c)
+  show ?case
+    unfolding rif.simps
+    apply (rule lfp_lowerbound)
+    using Loop(1)[OF finite_all_points, of "(varsL l |\<union>| Sup (vars ` P))" "(max (length l) (Pmax P))"] set_all_points_bound'[OF Loop(2), of l]
+    by auto    
+next
+  case (Parallel c1 c2)
+  show ?case unfolding rif.simps using set_all_points_bound'[OF Parallel(3)] by auto
+next
+  case (Thread c)
+  show ?case unfolding rif.simps using set_all_points_bound'[OF Thread(2)] by auto
+qed
+
+subsection \<open>While Rule\<close>
+
+lemma rif_While:
+  fixes b c P l
+  assumes "finite (P :: ('a, 'b) point set)"
+  defines "f == (\<lambda>Y. (P \<union> rif c l Y))"
+  shows "rif (Loop c) l P = while (\<lambda>Y. f Y \<noteq> Y) f {}" (is "_ = ?r")
+proof -
+  let ?V = "all_points (varsL l |\<union>| Sup (vars ` P)) (max (length l) (Pmax P)) :: ('a, 'b) point set"
+  have "lfp f = ?r"
+  proof(rule lfp_while[where C = "?V"])
+    show "mono f" using f_def mono_union_rif by blast
+  next
+    fix Y assume a: "Y \<subseteq> ?V"
+    have f: "finite Y" using a finite_all_points finite_subset by blast 
+    have "P \<subseteq> ?V" using set_all_points_bound' assms(1) by blast
+    moreover have "SimAsm_Inter.rif c l Y \<subseteq> ?V"
+      using rif_bound[OF f, of c l] all_points_const[OF all_points_sub[OF a]] by force
+    ultimately show "f Y \<subseteq> ?V" unfolding f_def by blast
+  next
+    show "finite ?V" by (rule finite_all_points)
+  qed
+  thus ?thesis unfolding f_def rif.simps(3) by blast
+qed
+
+lemma rif_While_let: "finite X \<Longrightarrow> rif (Loop c) l X =
+  (let f = (\<lambda>Y. X \<union> rif c l Y) in while (\<lambda>Y. f Y \<noteq> Y) f {})"
+  by (simp add: rif_While)
+
+lemma rif_While_set: "rif (Loop c) l (set xs) =
+  (let f = (\<lambda>Y. set xs \<union> rif c l Y) in while (\<lambda>Y. f Y \<noteq> Y) f {})"
+  by (rule rif_While_let, simp)
+
+lemmas [code] = rif.simps(1,2,4,5,6,7) rif_While_set
+
+section \<open>fset Execution\<close>
+
+text \<open>List implementation of fset, similar to that of set\<close>
+
+code_datatype fset_of_list
+
+lemma fset_empty [code]:
+  "{||} = fset_of_list []"
+  by simp
+
+lemma fset_insert [code]:
+  "finsert a (fset_of_list x) = fset_of_list (List.insert a x)"
+  by (simp add: List.insert_def finsert_absorb fset_of_list_elem)
+
+lemma fset_union [code]:
+  "fset_of_list a |\<union>| fset_of_list b = fset_of_list (List.union a b)"
+  by (metis fset_of_list.abs_eq fset_of_list_append set_append set_union)
+
+lemma fset_inter [code]:
+  "A |\<inter>| fset_of_list xs = fset_of_list (List.filter (\<lambda>x. x |\<in>| A) xs)"
+  by auto
+
+lemma fset_remove [code]:
+  "fset_of_list xs |-| A = fset_of_list (List.filter (\<lambda>x. x |\<notin>| A) xs)"
+  by auto
+
+lemma fset_hasGlobal [code]:
+  "hasGlobal (fset_of_list a) = hasGlobalL a"
+  by (induct a) (auto simp: hasGlobal_def; case_tac a1, auto)+
+
+lemma fset_mem [code]:
+  "(x |\<in>| fset_of_list F) = (List.member F x)"
+  by (simp add: fset_of_list_elem member_def)
+
+lemma fset_subset [code]:
+  "fset_of_list xs \<le> B \<longleftrightarrow> (\<forall>x\<in>set xs. x |\<in>| B)"
+  using fset_of_list.rep_eq notin_fset by fastforce
+
+declare fset_of_list_simps [code_post]
+
+section \<open>Tactics\<close>
+
+text \<open>Tactic to match the executable analysis within more abstract properties\<close>
+
+attribute_setup get_conv = \<open>Args.term >> (fn t =>
+        Thm.rule_attribute [] (fn context => fn _ =>
+          (Code_Simp.dynamic_conv (Context.proof_of context) o Thm.cterm_of (Context.proof_of context)) t))\<close>
+
+method rif_eval = 
+  (simp add: rif_checks_def rif_full_def del: rif.simps(1,2,4,5,6,7);
+   match conclusion in "checks l (rif c l' {}) R" for c and R 
+      and l :: "('a :: equal \<times>
+    ('b :: equal, 'c :: equal, 'd :: equal) op \<times>
+    (('b, ('c, 'd) SimAsm.var, 'e) state_rec_scheme
+     \<Rightarrow> 'e)) list"
+      and l' :: "('b :: equal, 'c  :: equal, 'd  :: equal) op list" \<Rightarrow>
+    \<open>match [[get_conv "rif c l' {}"]] in U: _ \<Rightarrow> \<open>subst U\<close>\<close>)
+
+end
